09ChainedEnvironment/ChainedEnvironment.thy
@@ -2,64 +2,85 @@ theory ChainedEnvironment
   imports "../07ByteCode/ByteCode" "../08HeapMemory/Heap"
 begin
 
-datatype ceclosure = 
-  CEConst nat
-  | CELam ptr nat
+section \<open>Chained environments\<close>
 
-datatype chained_state = 
-  CES "ceclosure heap" "(ptr \<times> ptr) heap" "ptr list" "(ptr \<times> nat) list"
+text \<open>We still have one place where information is duplicated: our environments themselves. They now 
+consist of lists of pointers rather than lists of values, but we still copy the list every time we 
+create a new function closure. At first we might think we could resolve this with the same trick we 
+used last stage, of storing the environments in the heap (or a new heap) and simply sharing pointers
+to them, but in fact this will not work. The problem is that unlike values, which once created never 
+change, an environment stored in a closure can be extended - and since a function closure can be 
+applied multiple times, extended in different ways.\<close>
+
+text \<open>We actually face a choice here. We could commit to copying the list every time, as a 
+contiguous block of data; this would be expensive every time a closure was copied, and mean that 
+closures occupy a varying (though compile-time-predictable) amount of space; but, as a consolation,
+variable lookup becomes very cheap (just a single pointer indirection). Alternately, we could store 
+environments as linked lists, making copying cheap and environments easy to extend in multiple 
+directions at once, but at the cost of making variable lookups expensive (a sequence of pointer 
+indirections proportional to their Debruijn index).\<close>
+
+text \<open>We will take the latter approach. We create a second heap, containing a linked-list (or 
+rather, pointer-linked tree) of pointers into our first, value, heap. All environments are now 
+pointers into this second heap, which means that our heaps point to each other; we keep them 
+separate for simplicity, although later on we will collapse them into a single memory.\<close>
+
+text \<open>To begin with, we define a lookup function for our linked-tree environments. Since we index 
+from the leaves towards the root, we don't actually have to deal with the tree structure; each 
+lookup looks like a list. We also distinguish a null pointer, 0, and therefore have to use \<open>Suc p\<close> 
+as a pointer to \<open>p\<close>.\<close>
 
 fun chain_lookup :: "('a \<times> ptr) heap \<Rightarrow> ptr \<Rightarrow> nat \<rightharpoonup> 'a" where
   "chain_lookup h 0 x = None"
-| "chain_lookup h (Suc p) 0 = Some (case hlookup h p of (a, b) \<Rightarrow> a)"
-| "chain_lookup h (Suc p) (Suc x) = chain_lookup h (case hlookup h p of (a, b) \<Rightarrow> b) x"
+| "chain_lookup h (Suc p) 0 = Some (fst (hlookup h p))"
+| "chain_lookup h (Suc p) (Suc x) = chain_lookup h (snd (hlookup h p)) x"
 
-inductive evalce :: "code\<^sub>b list \<Rightarrow> chained_state \<Rightarrow> chained_state \<Rightarrow> bool" 
-    (infix "\<tturnstile> _ \<leadsto>\<^sub>c\<^sub>e" 50) where
-  evce_lookup [simp]: "lookup cd pc = Some (Lookup\<^sub>b x) \<Longrightarrow> chain_lookup env p x = Some v \<Longrightarrow>
-    cd \<tturnstile> CES h env vs ((p, Suc pc) # sfs) \<leadsto>\<^sub>c\<^sub>e CES h env (v # vs) ((p, pc) # sfs)"
-| evce_pushcon [simp]: "lookup cd pc = Some (PushCon\<^sub>b k) \<Longrightarrow> halloc h (CEConst k) = (h', v) \<Longrightarrow>
-    cd \<tturnstile> CES h env vs ((p, Suc pc) # sfs) \<leadsto>\<^sub>c\<^sub>e CES h' env (v # vs) ((p, pc) # sfs)"
-| evce_pushlam [simp]: "lookup cd pc = Some (PushLam\<^sub>b pc') \<Longrightarrow> 
-    halloc h (CELam p pc') = (h', v) \<Longrightarrow> 
-      cd \<tturnstile> CES h env vs ((p, Suc pc) # sfs) \<leadsto>\<^sub>c\<^sub>e CES h' env (v # vs) ((p, pc) # sfs)"
-| evce_apply [simp]: "lookup cd pc = Some Apply\<^sub>b \<Longrightarrow> hlookup h v2 = CELam p' pc' \<Longrightarrow>
-    halloc env (v1, p') = (env', p'') \<Longrightarrow> 
-      cd \<tturnstile> CES h env (v1 # v2 # vs) ((p, Suc pc) # sfs) \<leadsto>\<^sub>c\<^sub>e 
-        CES h env' vs ((Suc p'', pc') # (p, pc) # sfs)"
-| evce_return [simp]: "lookup cd pc = Some Return\<^sub>b \<Longrightarrow> 
-    cd \<tturnstile> CES h env vs ((p, Suc pc) # sfs) \<leadsto>\<^sub>c\<^sub>e CES h env vs sfs"
-| evce_jump [simp]: "lookup cd pc = Some Jump\<^sub>b \<Longrightarrow> hlookup h v2 = CELam p' pc' \<Longrightarrow>
-    halloc env (v1, p') = (env', p'') \<Longrightarrow>
-      cd \<tturnstile> CES h env (v1 # v2 # vs) ((p, Suc pc) # sfs) \<leadsto>\<^sub>c\<^sub>e CES h env' vs ((Suc p'', pc') # sfs)"
+text \<open>From here, the new evaluation state and relation is simple. The only tricky point is to 
+remember that instead of just pushing values on top of the \<Delta>ironment in \<open>ev\<^sub>v_apply\<close> or \<open>ev\<^sub>v_jump\<close>,
+we must allocate a new cons cell (i.e., a pair) in the \<Delta>ironment heap.\<close>
 
-theorem determinismh: "cd \<tturnstile> \<Sigma> \<leadsto>\<^sub>c\<^sub>e \<Sigma>' \<Longrightarrow> cd \<tturnstile> \<Sigma> \<leadsto>\<^sub>c\<^sub>e \<Sigma>'' \<Longrightarrow> \<Sigma>' = \<Sigma>''"
-proof (induction \<Sigma> \<Sigma>' rule: evalce.induct)
-  case (evce_lookup cd pc x env p v h vs sfs)
-  from evce_lookup(3, 1, 2) show ?case 
-    by (induction cd "CES h env vs ((p, Suc pc) # sfs)" \<Sigma>'' rule: evalce.induct) simp_all 
+datatype closure\<^sub>v = 
+  Const\<^sub>v nat
+  | Lam\<^sub>v ptr nat
+
+datatype state\<^sub>v = 
+  S\<^sub>v "closure\<^sub>v heap" "(ptr \<times> ptr) heap" "ptr list" "(ptr \<times> nat) list"
+
+inductive eval\<^sub>v :: "code\<^sub>b list \<Rightarrow> state\<^sub>v \<Rightarrow> state\<^sub>v \<Rightarrow> bool" (infix "\<tturnstile> _ \<leadsto>\<^sub>v" 50) where
+  ev\<^sub>v_lookup [simp]: "lookup \<C> p\<^sub>\<C> = Some (Lookup\<^sub>b x) \<Longrightarrow> chain_lookup \<Delta> p\<^sub>\<Delta> x = Some v \<Longrightarrow>
+    \<C> \<tturnstile> S\<^sub>v h \<Delta> \<V> ((p\<^sub>\<Delta>, Suc p\<^sub>\<C>) # s) \<leadsto>\<^sub>v S\<^sub>v h \<Delta> (v # \<V>) ((p\<^sub>\<Delta>, p\<^sub>\<C>) # s)"
+| ev\<^sub>v_pushcon [simp]: "lookup \<C> p\<^sub>\<C> = Some (PushCon\<^sub>b n) \<Longrightarrow> halloc h (Const\<^sub>v n) = (h', v) \<Longrightarrow>
+    \<C> \<tturnstile> S\<^sub>v h \<Delta> \<V> ((p\<^sub>\<Delta>, Suc p\<^sub>\<C>) # s) \<leadsto>\<^sub>v S\<^sub>v h' \<Delta> (v # \<V>) ((p\<^sub>\<Delta>, p\<^sub>\<C>) # s)"
+| ev\<^sub>v_pushlam [simp]: "lookup \<C> p\<^sub>\<C> = Some (PushLam\<^sub>b p\<^sub>\<C>') \<Longrightarrow> halloc h (Lam\<^sub>v p\<^sub>\<Delta> p\<^sub>\<C>') = (h', v) \<Longrightarrow> 
+      \<C> \<tturnstile> S\<^sub>v h \<Delta> \<V> ((p\<^sub>\<Delta>, Suc p\<^sub>\<C>) # s) \<leadsto>\<^sub>v S\<^sub>v h' \<Delta> (v # \<V>) ((p\<^sub>\<Delta>, p\<^sub>\<C>) # s)"
+| ev\<^sub>v_apply [simp]: "lookup \<C> p\<^sub>\<C> = Some Apply\<^sub>b \<Longrightarrow> hlookup h v\<^sub>2 = Lam\<^sub>v p\<^sub>\<Delta>' p\<^sub>\<C>' \<Longrightarrow>
+    halloc \<Delta> (v\<^sub>1, p\<^sub>\<Delta>') = (\<Delta>', p\<^sub>\<Delta>'') \<Longrightarrow> 
+      \<C> \<tturnstile> S\<^sub>v h \<Delta> (v\<^sub>1 # v\<^sub>2 # \<V>) ((p\<^sub>\<Delta>, Suc p\<^sub>\<C>) # s) \<leadsto>\<^sub>v S\<^sub>v h \<Delta>' \<V> ((Suc p\<^sub>\<Delta>'', p\<^sub>\<C>') # (p\<^sub>\<Delta>, p\<^sub>\<C>) # s)"
+| ev\<^sub>v_return [simp]: "lookup \<C> p\<^sub>\<C> = Some Return\<^sub>b \<Longrightarrow> 
+    \<C> \<tturnstile> S\<^sub>v h \<Delta> \<V> ((p\<^sub>\<Delta>, Suc p\<^sub>\<C>) # s) \<leadsto>\<^sub>v S\<^sub>v h \<Delta> \<V> s"
+| ev\<^sub>v_jump [simp]: "lookup \<C> p\<^sub>\<C> = Some Jump\<^sub>b \<Longrightarrow> hlookup h v\<^sub>2 = Lam\<^sub>v p\<^sub>\<Delta>' p\<^sub>\<C>' \<Longrightarrow>
+    halloc \<Delta> (v\<^sub>1, p\<^sub>\<Delta>') = (\<Delta>', p\<^sub>\<Delta>'') \<Longrightarrow>
+      \<C> \<tturnstile> S\<^sub>v h \<Delta> (v\<^sub>1 # v\<^sub>2 # \<V>) ((p\<^sub>\<Delta>, Suc p\<^sub>\<C>) # s) \<leadsto>\<^sub>v S\<^sub>v h \<Delta>' \<V> ((Suc p\<^sub>\<Delta>'', p\<^sub>\<C>') # s)"
+
+theorem determinismh: "\<C> \<tturnstile> \<Sigma> \<leadsto>\<^sub>v \<Sigma>' \<Longrightarrow> \<C> \<tturnstile> \<Sigma> \<leadsto>\<^sub>v \<Sigma>'' \<Longrightarrow> \<Sigma>' = \<Sigma>''"
+proof (induction \<Sigma> \<Sigma>' rule: eval\<^sub>v.induct)
+  case ev\<^sub>v_lookup
+  from ev\<^sub>v_lookup(3, 1, 2) show ?case by (induction rule: eval\<^sub>v.cases) simp_all 
 next
-  case (evce_pushcon cd pc k h h' v env vs p sfs)
-  from evce_pushcon(3, 1, 2) show ?case 
-    by (induction cd "CES h env vs ((p, Suc pc) # sfs)" \<Sigma>'' rule: evalce.induct) simp_all 
+  case ev\<^sub>v_pushcon
+  from ev\<^sub>v_pushcon(3, 1, 2) show ?case by (induction rule: eval\<^sub>v.cases) simp_all 
 next
-  case (evce_pushlam cd pc pc' h p h' v env vs sfs)
-  from evce_pushlam(3, 1, 2) show ?case 
-    by (induction cd "CES h env vs ((p, Suc pc) # sfs)" \<Sigma>'' rule: evalce.induct) simp_all 
+  case ev\<^sub>v_pushlam
+  from ev\<^sub>v_pushlam(3, 1, 2) show ?case by (induction rule: eval\<^sub>v.cases) simp_all 
 next
-  case (evce_apply cd pc h v2 p' pc' env v1 env' p'' vs p sfs)
-  from evce_apply(4, 1, 2, 3) show ?case 
-    by (induction cd "CES h env (v1 # v2 # vs) ((p, Suc pc) # sfs)" \<Sigma>'' rule: evalce.induct) 
-       simp_all 
+  case ev\<^sub>v_apply
+  from ev\<^sub>v_apply(4, 1, 2, 3) show ?case by (induction rule: eval\<^sub>v.cases) simp_all 
 next
-  case (evce_return cd pc h env vs p sfs)
-  from evce_return(2, 1) show ?case 
-    by (induction cd "CES h env vs ((p, Suc pc) # sfs)" \<Sigma>'' rule: evalce.induct) simp_all 
+  case ev\<^sub>v_return
+  from ev\<^sub>v_return(2, 1) show ?case by (induction rule: eval\<^sub>v.cases) simp_all 
 next
-  case (evce_jump cd pc h v2 p' pc' env v1 env' p'' vs p sfs)
-  from evce_jump(4, 1, 2, 3) show ?case 
-    by (induction cd "CES h env (v1 # v2 # vs) ((p, Suc pc) # sfs)" \<Sigma>'' rule: evalce.induct) 
-       simp_all 
+  case ev\<^sub>v_jump
+  from ev\<^sub>v_jump(4, 1, 2, 3) show ?case by (induction rule: eval\<^sub>v.cases) simp_all 
 qed
 
 end
