09ChainedEnvironment/Chaining.thy
@@ -2,31 +2,33 @@ theory Chaining
   imports ChainedEnvironment "../08HeapMemory/HeapMemory"
 begin
 
-abbreviation chain_structured :: "ceclosure heap \<Rightarrow> (ptr \<times> ptr) heap \<Rightarrow> bool" where
+section \<open>Converting environments to chained form \<close>
+
+abbreviation chain_structured :: "closure\<^sub>v heap \<Rightarrow> (ptr \<times> ptr) heap \<Rightarrow> bool" where
   "chain_structured h env \<equiv> heap_all (\<lambda>p (v, p'). p' \<le> p \<and> hcontains h v) env"
 
 primrec chained_stack_pointer :: "(ptr \<times> ptr) heap \<Rightarrow> ptr \<Rightarrow> bool" where
   "chained_stack_pointer env 0 = True"
 | "chained_stack_pointer env (Suc p) = hcontains env p"
 
-fun chained_frame :: "(ptr \<times> ptr) heap \<Rightarrow> (ptr \<times> nat) \<Rightarrow> bool" where
+primrec chained_frame :: "(ptr \<times> ptr) heap \<Rightarrow> (ptr \<times> nat) \<Rightarrow> bool" where
   "chained_frame env (p, pc) = chained_stack_pointer env p"
 
 abbreviation chained_stack :: "(ptr \<times> ptr) heap \<Rightarrow> (ptr \<times> nat) list \<Rightarrow> bool" where
   "chained_stack env sfs \<equiv> list_all (chained_frame env) sfs"
 
-abbreviation chained_vals :: "ceclosure heap \<Rightarrow> ptr list \<Rightarrow> bool" where
+abbreviation chained_vals :: "closure\<^sub>v heap \<Rightarrow> ptr list \<Rightarrow> bool" where
   "chained_vals h vs \<equiv> list_all (hcontains h) vs"
 
-primrec chained_closure :: "(ptr \<times> ptr) heap \<Rightarrow> ceclosure \<Rightarrow> bool" where
-  "chained_closure env (CEConst n) = True"
-| "chained_closure env (CELam p pc) = chained_frame env (p, pc)"
+primrec chained_closure :: "(ptr \<times> ptr) heap \<Rightarrow> closure\<^sub>v \<Rightarrow> bool" where
+  "chained_closure env (Const\<^sub>v n) = True"
+| "chained_closure env (Lam\<^sub>v p pc) = chained_frame env (p, pc)"
 
-abbreviation chained_closures :: "(ptr \<times> ptr) heap \<Rightarrow> ceclosure heap \<Rightarrow> bool" where
+abbreviation chained_closures :: "(ptr \<times> ptr) heap \<Rightarrow> closure\<^sub>v heap \<Rightarrow> bool" where
   "chained_closures env h \<equiv> heap_all (\<lambda>p. chained_closure env) h"
 
-primrec chained_state :: "chained_state \<Rightarrow> bool" where
-  "chained_state (CES h env vs sfs) = (
+primrec chained_state :: "state\<^sub>v \<Rightarrow> bool" where
+  "chained_state (S\<^sub>v h env vs sfs) = (
     chain_structured h env \<and> chained_closures env h \<and> chained_vals h vs \<and> chained_stack env sfs)"
 
 fun unstack_list :: "(ptr \<times> ptr) heap \<Rightarrow> ptr \<Rightarrow> ptr list" where
@@ -34,11 +36,11 @@ fun unstack_list :: "(ptr \<times> ptr) heap \<Rightarrow> ptr \<Rightarrow> ptr
 | "unstack_list env (Suc p) = (case hlookup env p of 
       (v, p') \<Rightarrow> v # (if p' \<le> p then unstack_list env p' else undefined))"
 
-primrec unchain_closure :: "(ptr \<times> ptr) heap \<Rightarrow> ceclosure \<Rightarrow> closure\<^sub>h" where
-  "unchain_closure env (CEConst k) = Const\<^sub>h k"
-| "unchain_closure env (CELam p pc) = Lam\<^sub>h (unstack_list env p) pc"
+primrec unchain_closure :: "(ptr \<times> ptr) heap \<Rightarrow> closure\<^sub>v \<Rightarrow> closure\<^sub>h" where
+  "unchain_closure env (Const\<^sub>v k) = Const\<^sub>h k"
+| "unchain_closure env (Lam\<^sub>v p pc) = Lam\<^sub>h (unstack_list env p) pc"
 
-definition unchain_heap :: "ceclosure heap \<Rightarrow> (ptr \<times> ptr) heap \<Rightarrow> closure\<^sub>h heap" where
+definition unchain_heap :: "closure\<^sub>v heap \<Rightarrow> (ptr \<times> ptr) heap \<Rightarrow> closure\<^sub>h heap" where
   "unchain_heap h env = hmap (unchain_closure env) h"
 
 primrec unchain_frame :: "(ptr \<times> ptr) heap \<Rightarrow> (ptr \<times> nat) \<Rightarrow> (ptr list \<times> nat)" where
@@ -47,8 +49,8 @@ primrec unchain_frame :: "(ptr \<times> ptr) heap \<Rightarrow> (ptr \<times> na
 definition unchain_stack :: "(ptr \<times> ptr) heap \<Rightarrow> (ptr \<times> nat) list \<Rightarrow> (ptr list \<times> nat) list" where
   "unchain_stack env sfs = map (unchain_frame env) sfs"
 
-primrec unchain_state :: "chained_state \<Rightarrow> heap_state" where
-  "unchain_state (CES h env vs sfs) = S\<^sub>h (unchain_heap h env) vs (unchain_stack env sfs)"
+primrec unchain_state :: "state\<^sub>v \<Rightarrow> state\<^sub>h" where
+  "unchain_state (S\<^sub>v h env vs sfs) = S\<^sub>h (unchain_heap h env) vs (unchain_stack env sfs)"
 
 lemma [simp]: "chain_structured h env \<Longrightarrow> 
   heap_all (\<lambda>p (y, p'). p' \<le> p \<and> (y = x \<or> hcontains h y)) env"
@@ -111,43 +113,43 @@ proof (induction env p x rule: chain_lookup.induct)
   obtain v p' where V: "hlookup env p = (v, p')" by (cases "hlookup env p")
   from 3 have "hcontains env p" by auto
   with 3 V have P: "p' \<le> p" using hlookup_all by fast
-  with 3 have "chained_stack_pointer env p'" by auto
+  with 3 V have "chained_stack_pointer env p'" by auto
   with 3(1, 2) V P show ?case by fastforce
 qed (simp_all split: prod.splits)
 
-lemma [simp]: "halloc h (CEConst k) = (h', p) \<Longrightarrow> 
+lemma [simp]: "halloc h (Const\<^sub>v k) = (h', p) \<Longrightarrow> 
   halloc (unchain_heap h env) (Const\<^sub>h k) = (unchain_heap h' env, p)"
 proof -
-  assume "halloc h (CEConst k) = (h', p)"
-  hence "halloc (hmap (unchain_closure env) h) (unchain_closure env (CEConst k)) = 
+  assume "halloc h (Const\<^sub>v k) = (h', p)"
+  hence "halloc (hmap (unchain_closure env) h) (unchain_closure env (Const\<^sub>v k)) = 
     (hmap (unchain_closure env) h', p)" by (metis halloc_map)
   thus ?thesis by (simp add: unchain_heap_def)
 qed
 
-lemma [simp]: "halloc h (CELam p pc) = (h', v) \<Longrightarrow> 
+lemma [simp]: "halloc h (Lam\<^sub>v p pc) = (h', v) \<Longrightarrow> 
   halloc (unchain_heap h env) (Lam\<^sub>h (unstack_list env p) pc) = (unchain_heap h' env, v)"
 proof -
-  assume "halloc h (CELam p pc) = (h', v)"
-  hence "halloc (hmap (unchain_closure env) h) (unchain_closure env (CELam p pc)) = 
+  assume "halloc h (Lam\<^sub>v p pc) = (h', v)"
+  hence "halloc (hmap (unchain_closure env) h) (unchain_closure env (Lam\<^sub>v p pc)) = 
     (hmap (unchain_closure env) h', v)" by (metis halloc_map)
   thus ?thesis by (simp add: unchain_heap_def)
 qed
 
-lemma [simp]: "hlookup h x = CEConst k \<Longrightarrow> hcontains h x \<Longrightarrow> 
+lemma [simp]: "hlookup h x = Const\<^sub>v k \<Longrightarrow> hcontains h x \<Longrightarrow> 
     hlookup (unchain_heap h env) x = Const\<^sub>h k"
   by (simp add: unchain_heap_def)
 
-lemma [simp]: "hlookup h x = CELam p pc \<Longrightarrow> hcontains h x \<Longrightarrow> 
+lemma [simp]: "hlookup h x = Lam\<^sub>v p pc \<Longrightarrow> hcontains h x \<Longrightarrow> 
     hlookup (unchain_heap h env) x = Lam\<^sub>h (unstack_list env p) pc"
   by (simp add: unchain_heap_def)
 
 lemma unchain_state_reverse [dest]: "S\<^sub>h h vs sfs = unchain_state \<Sigma> \<Longrightarrow> 
-  \<exists>h\<^sub>c\<^sub>e env sfs\<^sub>c\<^sub>e. \<Sigma> = CES h\<^sub>c\<^sub>e env vs sfs\<^sub>c\<^sub>e \<and> h = unchain_heap h\<^sub>c\<^sub>e env \<and> 
+  \<exists>h\<^sub>c\<^sub>e env sfs\<^sub>c\<^sub>e. \<Sigma> = S\<^sub>v h\<^sub>c\<^sub>e env vs sfs\<^sub>c\<^sub>e \<and> h = unchain_heap h\<^sub>c\<^sub>e env \<and> 
     sfs = unchain_stack env sfs\<^sub>c\<^sub>e"
   by (induction \<Sigma>) simp_all
 
 lemma [dest]: "Lam\<^sub>h env\<^sub>h pc = unchain_closure env\<^sub>c\<^sub>e x \<Longrightarrow> 
-    \<exists>p. x = CELam p pc \<and> env\<^sub>h = unstack_list env\<^sub>c\<^sub>e p"
+    \<exists>p. x = Lam\<^sub>v p pc \<and> env\<^sub>h = unstack_list env\<^sub>c\<^sub>e p"
   by (induction x) simp_all
 
 lemma [elim]: "hcontains env p \<Longrightarrow> halloc env v = (env', q) \<Longrightarrow> 
@@ -174,9 +176,9 @@ proof (unfold unchain_heap_def)
     assume X: "hcontains h x"
     show "unchain_closure env' (hlookup h x) = unchain_closure env (hlookup h x)" 
     proof (cases "hlookup h x")
-      case (CELam pp pc)
-      with C X have "chained_closure env (CELam pp pc)" by (metis hlookup_all)
-      with S A CELam show ?thesis by auto
+      case (Lam\<^sub>v pp pc)
+      with C X have "chained_closure env (Lam\<^sub>v pp pc)" by (metis hlookup_all)
+      with S A Lam\<^sub>v show ?thesis by auto
     qed simp_all
   qed
   thus "hmap (unchain_closure env') h = hmap (unchain_closure env) h" by (metis hmap_eq)
@@ -200,66 +202,66 @@ lemma [elim]: "chained_stack env sfs \<Longrightarrow> halloc env v = (env', p) 
   by (induction sfs) (auto simp add: unchain_stack_def)
 
 theorem completece [simp]: "cd \<tturnstile> unchain_state \<Sigma>\<^sub>c\<^sub>e \<leadsto>\<^sub>h \<Sigma>\<^sub>h \<Longrightarrow> chained_state \<Sigma>\<^sub>c\<^sub>e \<Longrightarrow>
-  \<exists>\<Sigma>\<^sub>c\<^sub>e'. (cd \<tturnstile> \<Sigma>\<^sub>c\<^sub>e \<leadsto>\<^sub>c\<^sub>e \<Sigma>\<^sub>c\<^sub>e') \<and> \<Sigma>\<^sub>h = unchain_state \<Sigma>\<^sub>c\<^sub>e'"
+  \<exists>\<Sigma>\<^sub>c\<^sub>e'. (cd \<tturnstile> \<Sigma>\<^sub>c\<^sub>e \<leadsto>\<^sub>v \<Sigma>\<^sub>c\<^sub>e') \<and> \<Sigma>\<^sub>h = unchain_state \<Sigma>\<^sub>c\<^sub>e'"
 proof (induction "unchain_state \<Sigma>\<^sub>c\<^sub>e" \<Sigma>\<^sub>h arbitrary: \<Sigma>\<^sub>c\<^sub>e rule: eval\<^sub>h.induct)
   case (ev\<^sub>h_lookup cd pc x env v h vs sfs)
-  then obtain h\<^sub>c\<^sub>e env\<^sub>c\<^sub>e sfs\<^sub>c\<^sub>e' where S: "\<Sigma>\<^sub>c\<^sub>e = CES h\<^sub>c\<^sub>e env\<^sub>c\<^sub>e vs sfs\<^sub>c\<^sub>e' \<and> h = unchain_heap h\<^sub>c\<^sub>e env\<^sub>c\<^sub>e \<and> 
+  then obtain h\<^sub>c\<^sub>e env\<^sub>c\<^sub>e sfs\<^sub>c\<^sub>e' where S: "\<Sigma>\<^sub>c\<^sub>e = S\<^sub>v h\<^sub>c\<^sub>e env\<^sub>c\<^sub>e vs sfs\<^sub>c\<^sub>e' \<and> h = unchain_heap h\<^sub>c\<^sub>e env\<^sub>c\<^sub>e \<and> 
     (env, Suc pc) # sfs = unchain_stack env\<^sub>c\<^sub>e sfs\<^sub>c\<^sub>e'" by fastforce
   then obtain sf\<^sub>c\<^sub>e sfs\<^sub>c\<^sub>e where SF: "sfs\<^sub>c\<^sub>e' = sf\<^sub>c\<^sub>e # sfs\<^sub>c\<^sub>e \<and> (env, Suc pc) = unchain_frame env\<^sub>c\<^sub>e sf\<^sub>c\<^sub>e \<and> 
     sfs = unchain_stack env\<^sub>c\<^sub>e sfs\<^sub>c\<^sub>e" by (auto simp add: unchain_stack_def)
   then obtain p where P: "sf\<^sub>c\<^sub>e = (p, Suc pc) \<and> env = unstack_list env\<^sub>c\<^sub>e p" by (cases sf\<^sub>c\<^sub>e) simp_all
   with ev\<^sub>h_lookup S SF have C: "chain_structured h\<^sub>c\<^sub>e env\<^sub>c\<^sub>e" by simp
   with ev\<^sub>h_lookup S SF P have X: "S\<^sub>h h (v # vs) ((env, pc) # sfs) = 
-    unchain_state (CES h\<^sub>c\<^sub>e env\<^sub>c\<^sub>e (v # vs) ((p, pc) # sfs\<^sub>c\<^sub>e))" by (simp add: unchain_stack_def)
+    unchain_state (S\<^sub>v h\<^sub>c\<^sub>e env\<^sub>c\<^sub>e (v # vs) ((p, pc) # sfs\<^sub>c\<^sub>e))" by (simp add: unchain_stack_def)
   from ev\<^sub>h_lookup S SF P have "chained_frame env\<^sub>c\<^sub>e (p, Suc pc)" by simp
   with C have "lookup (unstack_list env\<^sub>c\<^sub>e p) x = chain_lookup env\<^sub>c\<^sub>e p x" by simp
-  with ev\<^sub>h_lookup P C have "cd \<tturnstile> CES h\<^sub>c\<^sub>e env\<^sub>c\<^sub>e vs ((p, Suc pc) # sfs\<^sub>c\<^sub>e) \<leadsto>\<^sub>c\<^sub>e 
-    CES h\<^sub>c\<^sub>e env\<^sub>c\<^sub>e (v # vs) ((p, pc) # sfs\<^sub>c\<^sub>e)" by simp
+  with ev\<^sub>h_lookup P C have "cd \<tturnstile> S\<^sub>v h\<^sub>c\<^sub>e env\<^sub>c\<^sub>e vs ((p, Suc pc) # sfs\<^sub>c\<^sub>e) \<leadsto>\<^sub>v 
+    S\<^sub>v h\<^sub>c\<^sub>e env\<^sub>c\<^sub>e (v # vs) ((p, pc) # sfs\<^sub>c\<^sub>e)" by simp
   with S SF P X show ?case by blast
 next
   case (ev\<^sub>h_pushcon cd pc k h h' v vs env sfs)
-  then obtain h\<^sub>c\<^sub>e env\<^sub>c\<^sub>e sfs\<^sub>c\<^sub>e' where S: "\<Sigma>\<^sub>c\<^sub>e = CES h\<^sub>c\<^sub>e env\<^sub>c\<^sub>e vs sfs\<^sub>c\<^sub>e' \<and> h = unchain_heap h\<^sub>c\<^sub>e env\<^sub>c\<^sub>e \<and> 
+  then obtain h\<^sub>c\<^sub>e env\<^sub>c\<^sub>e sfs\<^sub>c\<^sub>e' where S: "\<Sigma>\<^sub>c\<^sub>e = S\<^sub>v h\<^sub>c\<^sub>e env\<^sub>c\<^sub>e vs sfs\<^sub>c\<^sub>e' \<and> h = unchain_heap h\<^sub>c\<^sub>e env\<^sub>c\<^sub>e \<and> 
     (env, Suc pc) # sfs = unchain_stack env\<^sub>c\<^sub>e sfs\<^sub>c\<^sub>e'" by fastforce
   then obtain sf\<^sub>c\<^sub>e sfs\<^sub>c\<^sub>e where SF: "sfs\<^sub>c\<^sub>e' = sf\<^sub>c\<^sub>e # sfs\<^sub>c\<^sub>e \<and> (env, Suc pc) = unchain_frame env\<^sub>c\<^sub>e sf\<^sub>c\<^sub>e \<and> 
     sfs = unchain_stack env\<^sub>c\<^sub>e sfs\<^sub>c\<^sub>e" by (auto simp add: unchain_stack_def)
   then obtain p where P: "sf\<^sub>c\<^sub>e = (p, Suc pc) \<and> env = unstack_list env\<^sub>c\<^sub>e p" by (cases sf\<^sub>c\<^sub>e) simp_all
   from ev\<^sub>h_pushcon S have "halloc (hmap (unchain_closure env\<^sub>c\<^sub>e) h\<^sub>c\<^sub>e) 
-    (unchain_closure env\<^sub>c\<^sub>e (CEConst k)) = (h', v)" by (simp add: unchain_heap_def)
-  then obtain h\<^sub>c\<^sub>e' where H: "halloc h\<^sub>c\<^sub>e (CEConst k) = (h\<^sub>c\<^sub>e', v) \<and> 
+    (unchain_closure env\<^sub>c\<^sub>e (Const\<^sub>v k)) = (h', v)" by (simp add: unchain_heap_def)
+  then obtain h\<^sub>c\<^sub>e' where H: "halloc h\<^sub>c\<^sub>e (Const\<^sub>v k) = (h\<^sub>c\<^sub>e', v) \<and> 
     h' = hmap (unchain_closure env\<^sub>c\<^sub>e) h\<^sub>c\<^sub>e'" by (metis halloc_map_inv)
   hence "h' = unchain_heap h\<^sub>c\<^sub>e' env\<^sub>c\<^sub>e" by (simp add: unchain_heap_def)
   with SF P have X: "S\<^sub>h h' (v # vs) ((env, pc) # sfs) = 
-    unchain_state (CES h\<^sub>c\<^sub>e' env\<^sub>c\<^sub>e (v # vs) ((p, pc) # sfs\<^sub>c\<^sub>e))" by (simp add: unchain_stack_def)
-  from ev\<^sub>h_pushcon H have "cd \<tturnstile> CES h\<^sub>c\<^sub>e env\<^sub>c\<^sub>e vs ((p, Suc pc) # sfs\<^sub>c\<^sub>e) \<leadsto>\<^sub>c\<^sub>e 
-    CES h\<^sub>c\<^sub>e' env\<^sub>c\<^sub>e (v # vs) ((p, pc) # sfs\<^sub>c\<^sub>e)" by simp
+    unchain_state (S\<^sub>v h\<^sub>c\<^sub>e' env\<^sub>c\<^sub>e (v # vs) ((p, pc) # sfs\<^sub>c\<^sub>e))" by (simp add: unchain_stack_def)
+  from ev\<^sub>h_pushcon H have "cd \<tturnstile> S\<^sub>v h\<^sub>c\<^sub>e env\<^sub>c\<^sub>e vs ((p, Suc pc) # sfs\<^sub>c\<^sub>e) \<leadsto>\<^sub>v 
+    S\<^sub>v h\<^sub>c\<^sub>e' env\<^sub>c\<^sub>e (v # vs) ((p, pc) # sfs\<^sub>c\<^sub>e)" by simp
   with S SF P X show ?case by blast
 next
   case (ev\<^sub>h_pushlam cd pc pc' h env h' v vs sfs)
-  then obtain h\<^sub>c\<^sub>e env\<^sub>c\<^sub>e sfs\<^sub>c\<^sub>e' where S: "\<Sigma>\<^sub>c\<^sub>e = CES h\<^sub>c\<^sub>e env\<^sub>c\<^sub>e vs sfs\<^sub>c\<^sub>e' \<and> h = unchain_heap h\<^sub>c\<^sub>e env\<^sub>c\<^sub>e \<and> 
+  then obtain h\<^sub>c\<^sub>e env\<^sub>c\<^sub>e sfs\<^sub>c\<^sub>e' where S: "\<Sigma>\<^sub>c\<^sub>e = S\<^sub>v h\<^sub>c\<^sub>e env\<^sub>c\<^sub>e vs sfs\<^sub>c\<^sub>e' \<and> h = unchain_heap h\<^sub>c\<^sub>e env\<^sub>c\<^sub>e \<and> 
     (env, Suc pc) # sfs = unchain_stack env\<^sub>c\<^sub>e sfs\<^sub>c\<^sub>e'" by fastforce
   then obtain sf\<^sub>c\<^sub>e sfs\<^sub>c\<^sub>e where SF: "sfs\<^sub>c\<^sub>e' = sf\<^sub>c\<^sub>e # sfs\<^sub>c\<^sub>e \<and> (env, Suc pc) = unchain_frame env\<^sub>c\<^sub>e sf\<^sub>c\<^sub>e \<and> 
     sfs = unchain_stack env\<^sub>c\<^sub>e sfs\<^sub>c\<^sub>e" by (auto simp add: unchain_stack_def)
   then obtain p where P: "sf\<^sub>c\<^sub>e = (p, Suc pc) \<and> env = unstack_list env\<^sub>c\<^sub>e p" by (cases sf\<^sub>c\<^sub>e) simp_all
   with ev\<^sub>h_pushlam S have "halloc (hmap (unchain_closure env\<^sub>c\<^sub>e) h\<^sub>c\<^sub>e) 
-    (unchain_closure env\<^sub>c\<^sub>e (CELam p pc')) = (h', v)" by (simp add: unchain_heap_def)
-  then obtain h\<^sub>c\<^sub>e' where H: "halloc h\<^sub>c\<^sub>e (CELam p pc') = (h\<^sub>c\<^sub>e', v) \<and> 
+    (unchain_closure env\<^sub>c\<^sub>e (Lam\<^sub>v p pc')) = (h', v)" by (simp add: unchain_heap_def)
+  then obtain h\<^sub>c\<^sub>e' where H: "halloc h\<^sub>c\<^sub>e (Lam\<^sub>v p pc') = (h\<^sub>c\<^sub>e', v) \<and> 
     h' = hmap (unchain_closure env\<^sub>c\<^sub>e) h\<^sub>c\<^sub>e'" by (metis halloc_map_inv)
   hence "h' = unchain_heap h\<^sub>c\<^sub>e' env\<^sub>c\<^sub>e" by (simp add: unchain_heap_def)
   with SF P have X: "S\<^sub>h h' (v # vs) ((env, pc) # sfs) = 
-    unchain_state (CES h\<^sub>c\<^sub>e' env\<^sub>c\<^sub>e (v # vs) ((p, pc) # sfs\<^sub>c\<^sub>e))" by (simp add: unchain_stack_def)
-  from ev\<^sub>h_pushlam H have "cd \<tturnstile> CES h\<^sub>c\<^sub>e env\<^sub>c\<^sub>e vs ((p, Suc pc) # sfs\<^sub>c\<^sub>e) \<leadsto>\<^sub>c\<^sub>e 
-    CES h\<^sub>c\<^sub>e' env\<^sub>c\<^sub>e (v # vs) ((p, pc) # sfs\<^sub>c\<^sub>e)" by simp
+    unchain_state (S\<^sub>v h\<^sub>c\<^sub>e' env\<^sub>c\<^sub>e (v # vs) ((p, pc) # sfs\<^sub>c\<^sub>e))" by (simp add: unchain_stack_def)
+  from ev\<^sub>h_pushlam H have "cd \<tturnstile> S\<^sub>v h\<^sub>c\<^sub>e env\<^sub>c\<^sub>e vs ((p, Suc pc) # sfs\<^sub>c\<^sub>e) \<leadsto>\<^sub>v 
+    S\<^sub>v h\<^sub>c\<^sub>e' env\<^sub>c\<^sub>e (v # vs) ((p, pc) # sfs\<^sub>c\<^sub>e)" by simp
   with S SF P X show ?case by blast
 next
   case (ev\<^sub>h_apply cd pc h v2 env' pc' v1 vs env sfs)
-  then obtain h\<^sub>c\<^sub>e env\<^sub>c\<^sub>e sfs\<^sub>c\<^sub>e' where S: "\<Sigma>\<^sub>c\<^sub>e = CES h\<^sub>c\<^sub>e env\<^sub>c\<^sub>e (v1 # v2 # vs) sfs\<^sub>c\<^sub>e' \<and> 
+  then obtain h\<^sub>c\<^sub>e env\<^sub>c\<^sub>e sfs\<^sub>c\<^sub>e' where S: "\<Sigma>\<^sub>c\<^sub>e = S\<^sub>v h\<^sub>c\<^sub>e env\<^sub>c\<^sub>e (v1 # v2 # vs) sfs\<^sub>c\<^sub>e' \<and> 
     h = unchain_heap h\<^sub>c\<^sub>e env\<^sub>c\<^sub>e \<and> (env, Suc pc) # sfs = unchain_stack env\<^sub>c\<^sub>e sfs\<^sub>c\<^sub>e'" by fastforce
   then obtain sf\<^sub>c\<^sub>e sfs\<^sub>c\<^sub>e where SF: "sfs\<^sub>c\<^sub>e' = sf\<^sub>c\<^sub>e # sfs\<^sub>c\<^sub>e \<and> (env, Suc pc) = unchain_frame env\<^sub>c\<^sub>e sf\<^sub>c\<^sub>e \<and> 
     sfs = unchain_stack env\<^sub>c\<^sub>e sfs\<^sub>c\<^sub>e" by (auto simp add: unchain_stack_def)
   then obtain p where P: "sf\<^sub>c\<^sub>e = (p, Suc pc) \<and> env = unstack_list env\<^sub>c\<^sub>e p" by (cases sf\<^sub>c\<^sub>e) simp_all
   from ev\<^sub>h_apply S have "Lam\<^sub>h env' pc' = unchain_closure env\<^sub>c\<^sub>e (hlookup h\<^sub>c\<^sub>e v2)" 
     by (simp add: unchain_heap_def)
-  then obtain p' where P': "hlookup h\<^sub>c\<^sub>e v2 = CELam p' pc' \<and> env' = unstack_list env\<^sub>c\<^sub>e p'" by blast
+  then obtain p' where P': "hlookup h\<^sub>c\<^sub>e v2 = Lam\<^sub>v p' pc' \<and> env' = unstack_list env\<^sub>c\<^sub>e p'" by blast
   obtain env\<^sub>c\<^sub>e' p'' where H: "halloc env\<^sub>c\<^sub>e (v1, p') = (env\<^sub>c\<^sub>e', p'')" 
     by (cases "halloc env\<^sub>c\<^sub>e (v1, p')") simp_all
   from ev\<^sub>h_apply S SF P have C: "chain_structured h\<^sub>c\<^sub>e env\<^sub>c\<^sub>e \<and> chained_closures env\<^sub>c\<^sub>e h\<^sub>c\<^sub>e \<and>
@@ -268,7 +270,7 @@ next
   with H have Y: "unchain_heap h\<^sub>c\<^sub>e env\<^sub>c\<^sub>e' = unchain_heap h\<^sub>c\<^sub>e env\<^sub>c\<^sub>e" by fast
   from H C have "unstack_list env\<^sub>c\<^sub>e' p = unstack_list env\<^sub>c\<^sub>e p" by fastforce
   with P have W: "env = unstack_list env\<^sub>c\<^sub>e' p" by metis
-  from P' C have "chained_closure env\<^sub>c\<^sub>e (CELam p' pc')" by (metis hlookup_all)
+  from P' C have "chained_closure env\<^sub>c\<^sub>e (Lam\<^sub>v p' pc')" by (metis hlookup_all)
   hence "chained_stack_pointer env\<^sub>c\<^sub>e p'" by auto
   with H C have "unstack_list env\<^sub>c\<^sub>e' (Suc p'') = v1 # unstack_list env\<^sub>c\<^sub>e p'" 
     by (metis unfold_unstack_list)
@@ -276,38 +278,38 @@ next
   from H C have "unchain_stack env\<^sub>c\<^sub>e' sfs\<^sub>c\<^sub>e = unchain_stack env\<^sub>c\<^sub>e sfs\<^sub>c\<^sub>e" by fast
   with SF have "sfs = unchain_stack env\<^sub>c\<^sub>e' sfs\<^sub>c\<^sub>e" by simp
   with S Y Z W have X: "S\<^sub>h h vs ((v1 # env', pc') # (env, pc) # sfs) = 
-    unchain_state (CES h\<^sub>c\<^sub>e env\<^sub>c\<^sub>e' vs ((Suc p'', pc') # (p, pc) # sfs\<^sub>c\<^sub>e))" 
+    unchain_state (S\<^sub>v h\<^sub>c\<^sub>e env\<^sub>c\<^sub>e' vs ((Suc p'', pc') # (p, pc) # sfs\<^sub>c\<^sub>e))" 
       by (simp add: unchain_stack_def)
-  from ev\<^sub>h_apply P' H have "cd \<tturnstile> CES h\<^sub>c\<^sub>e env\<^sub>c\<^sub>e (v1 # v2 # vs) ((p, Suc pc) # sfs\<^sub>c\<^sub>e) \<leadsto>\<^sub>c\<^sub>e 
-      CES h\<^sub>c\<^sub>e env\<^sub>c\<^sub>e' vs ((Suc p'', pc') # (p, pc) # sfs\<^sub>c\<^sub>e)" by simp
+  from ev\<^sub>h_apply P' H have "cd \<tturnstile> S\<^sub>v h\<^sub>c\<^sub>e env\<^sub>c\<^sub>e (v1 # v2 # vs) ((p, Suc pc) # sfs\<^sub>c\<^sub>e) \<leadsto>\<^sub>v 
+      S\<^sub>v h\<^sub>c\<^sub>e env\<^sub>c\<^sub>e' vs ((Suc p'', pc') # (p, pc) # sfs\<^sub>c\<^sub>e)" by simp
   with S SF P X show ?case by blast
 next
   case (ev\<^sub>h_return cd pc h vs env sfs)
-  then obtain h\<^sub>c\<^sub>e env\<^sub>c\<^sub>e sfs\<^sub>c\<^sub>e' where S: "\<Sigma>\<^sub>c\<^sub>e = CES h\<^sub>c\<^sub>e env\<^sub>c\<^sub>e vs sfs\<^sub>c\<^sub>e' \<and> h = unchain_heap h\<^sub>c\<^sub>e env\<^sub>c\<^sub>e \<and> 
+  then obtain h\<^sub>c\<^sub>e env\<^sub>c\<^sub>e sfs\<^sub>c\<^sub>e' where S: "\<Sigma>\<^sub>c\<^sub>e = S\<^sub>v h\<^sub>c\<^sub>e env\<^sub>c\<^sub>e vs sfs\<^sub>c\<^sub>e' \<and> h = unchain_heap h\<^sub>c\<^sub>e env\<^sub>c\<^sub>e \<and> 
     (env, Suc pc) # sfs = unchain_stack env\<^sub>c\<^sub>e sfs\<^sub>c\<^sub>e'" by fastforce
   then obtain sf\<^sub>c\<^sub>e sfs\<^sub>c\<^sub>e where SF: "sfs\<^sub>c\<^sub>e' = sf\<^sub>c\<^sub>e # sfs\<^sub>c\<^sub>e \<and> (env, Suc pc) = unchain_frame env\<^sub>c\<^sub>e sf\<^sub>c\<^sub>e \<and> 
     sfs = unchain_stack env\<^sub>c\<^sub>e sfs\<^sub>c\<^sub>e" by (auto simp add: unchain_stack_def)
   then obtain p where P: "sf\<^sub>c\<^sub>e = (p, Suc pc) \<and> env = unstack_list env\<^sub>c\<^sub>e p" by (cases sf\<^sub>c\<^sub>e) simp_all
-  from S SF have X: "S\<^sub>h h vs sfs = unchain_state (CES h\<^sub>c\<^sub>e env\<^sub>c\<^sub>e vs sfs\<^sub>c\<^sub>e)" by simp
-  from ev\<^sub>h_return have "cd \<tturnstile> CES h\<^sub>c\<^sub>e env\<^sub>c\<^sub>e vs ((p, Suc pc) # sfs\<^sub>c\<^sub>e) \<leadsto>\<^sub>c\<^sub>e CES h\<^sub>c\<^sub>e env\<^sub>c\<^sub>e vs sfs\<^sub>c\<^sub>e" by simp
+  from S SF have X: "S\<^sub>h h vs sfs = unchain_state (S\<^sub>v h\<^sub>c\<^sub>e env\<^sub>c\<^sub>e vs sfs\<^sub>c\<^sub>e)" by simp
+  from ev\<^sub>h_return have "cd \<tturnstile> S\<^sub>v h\<^sub>c\<^sub>e env\<^sub>c\<^sub>e vs ((p, Suc pc) # sfs\<^sub>c\<^sub>e) \<leadsto>\<^sub>v S\<^sub>v h\<^sub>c\<^sub>e env\<^sub>c\<^sub>e vs sfs\<^sub>c\<^sub>e" by simp
   with S SF P X show ?case by blast
 next
   case (ev\<^sub>h_jump cd pc h v2 env' pc' v1 vs env sfs)
-  then obtain h\<^sub>c\<^sub>e env\<^sub>c\<^sub>e sfs\<^sub>c\<^sub>e' where S: "\<Sigma>\<^sub>c\<^sub>e = CES h\<^sub>c\<^sub>e env\<^sub>c\<^sub>e (v1 # v2 # vs) sfs\<^sub>c\<^sub>e' \<and> 
+  then obtain h\<^sub>c\<^sub>e env\<^sub>c\<^sub>e sfs\<^sub>c\<^sub>e' where S: "\<Sigma>\<^sub>c\<^sub>e = S\<^sub>v h\<^sub>c\<^sub>e env\<^sub>c\<^sub>e (v1 # v2 # vs) sfs\<^sub>c\<^sub>e' \<and> 
     h = unchain_heap h\<^sub>c\<^sub>e env\<^sub>c\<^sub>e \<and> (env, Suc pc) # sfs = unchain_stack env\<^sub>c\<^sub>e sfs\<^sub>c\<^sub>e'" by fastforce
   then obtain sf\<^sub>c\<^sub>e sfs\<^sub>c\<^sub>e where SF: "sfs\<^sub>c\<^sub>e' = sf\<^sub>c\<^sub>e # sfs\<^sub>c\<^sub>e \<and> (env, Suc pc) = unchain_frame env\<^sub>c\<^sub>e sf\<^sub>c\<^sub>e \<and> 
     sfs = unchain_stack env\<^sub>c\<^sub>e sfs\<^sub>c\<^sub>e" by (auto simp add: unchain_stack_def)
   then obtain p where P: "sf\<^sub>c\<^sub>e = (p, Suc pc) \<and> env = unstack_list env\<^sub>c\<^sub>e p" by (cases sf\<^sub>c\<^sub>e) simp_all
   from ev\<^sub>h_jump S have "Lam\<^sub>h env' pc' = unchain_closure env\<^sub>c\<^sub>e (hlookup h\<^sub>c\<^sub>e v2)" 
     by (simp add: unchain_heap_def)
-  then obtain p' where P': "hlookup h\<^sub>c\<^sub>e v2 = CELam p' pc' \<and> env' = unstack_list env\<^sub>c\<^sub>e p'" by blast
+  then obtain p' where P': "hlookup h\<^sub>c\<^sub>e v2 = Lam\<^sub>v p' pc' \<and> env' = unstack_list env\<^sub>c\<^sub>e p'" by blast
   obtain env\<^sub>c\<^sub>e' p'' where H: "halloc env\<^sub>c\<^sub>e (v1, p') = (env\<^sub>c\<^sub>e', p'')" 
     by (cases "halloc env\<^sub>c\<^sub>e (v1, p')") simp_all
   from ev\<^sub>h_jump S SF P have C: "chain_structured h\<^sub>c\<^sub>e env\<^sub>c\<^sub>e \<and> chained_closures env\<^sub>c\<^sub>e h\<^sub>c\<^sub>e \<and>
     hcontains h\<^sub>c\<^sub>e v1 \<and> hcontains h\<^sub>c\<^sub>e v2 \<and> chained_vals h\<^sub>c\<^sub>e vs \<and> chained_stack_pointer env\<^sub>c\<^sub>e p \<and> 
       chained_stack env\<^sub>c\<^sub>e sfs\<^sub>c\<^sub>e" by simp
   with H have Y: "unchain_heap h\<^sub>c\<^sub>e env\<^sub>c\<^sub>e' = unchain_heap h\<^sub>c\<^sub>e env\<^sub>c\<^sub>e" by fast
-  from P' C have "chained_closure env\<^sub>c\<^sub>e (CELam p' pc')" by (metis hlookup_all)
+  from P' C have "chained_closure env\<^sub>c\<^sub>e (Lam\<^sub>v p' pc')" by (metis hlookup_all)
   hence "chained_stack_pointer env\<^sub>c\<^sub>e p'" by simp
   with H C have "unstack_list env\<^sub>c\<^sub>e' (Suc p'') = v1 # unstack_list env\<^sub>c\<^sub>e p'" 
     by (metis unfold_unstack_list)
@@ -315,44 +317,44 @@ next
   from H C have "unchain_stack env\<^sub>c\<^sub>e' sfs\<^sub>c\<^sub>e = unchain_stack env\<^sub>c\<^sub>e sfs\<^sub>c\<^sub>e" by fast
   with SF have "sfs = unchain_stack env\<^sub>c\<^sub>e' sfs\<^sub>c\<^sub>e" by simp
   with S Y Z have X: "S\<^sub>h h vs ((v1 # env', pc') # sfs) = 
-    unchain_state (CES h\<^sub>c\<^sub>e env\<^sub>c\<^sub>e' vs ((Suc p'', pc') # sfs\<^sub>c\<^sub>e))" by (simp add: unchain_stack_def)
-  from ev\<^sub>h_jump P' H have "cd \<tturnstile> CES h\<^sub>c\<^sub>e env\<^sub>c\<^sub>e (v1 # v2 # vs) ((p, Suc pc) # sfs\<^sub>c\<^sub>e) \<leadsto>\<^sub>c\<^sub>e 
-      CES h\<^sub>c\<^sub>e env\<^sub>c\<^sub>e' vs ((Suc p'', pc') # sfs\<^sub>c\<^sub>e)" by simp
+    unchain_state (S\<^sub>v h\<^sub>c\<^sub>e env\<^sub>c\<^sub>e' vs ((Suc p'', pc') # sfs\<^sub>c\<^sub>e))" by (simp add: unchain_stack_def)
+  from ev\<^sub>h_jump P' H have "cd \<tturnstile> S\<^sub>v h\<^sub>c\<^sub>e env\<^sub>c\<^sub>e (v1 # v2 # vs) ((p, Suc pc) # sfs\<^sub>c\<^sub>e) \<leadsto>\<^sub>v 
+      S\<^sub>v h\<^sub>c\<^sub>e env\<^sub>c\<^sub>e' vs ((Suc p'', pc') # sfs\<^sub>c\<^sub>e)" by simp
   with S SF P X show ?case by blast
 qed
 
-theorem correctce [simp]: "cd \<tturnstile> \<Sigma>\<^sub>c\<^sub>e \<leadsto>\<^sub>c\<^sub>e \<Sigma>\<^sub>c\<^sub>e' \<Longrightarrow> chained_state \<Sigma>\<^sub>c\<^sub>e \<Longrightarrow> 
+theorem correctce [simp]: "cd \<tturnstile> \<Sigma>\<^sub>c\<^sub>e \<leadsto>\<^sub>v \<Sigma>\<^sub>c\<^sub>e' \<Longrightarrow> chained_state \<Sigma>\<^sub>c\<^sub>e \<Longrightarrow> 
   cd \<tturnstile> unchain_state \<Sigma>\<^sub>c\<^sub>e \<leadsto>\<^sub>h unchain_state \<Sigma>\<^sub>c\<^sub>e'"
-proof (induction \<Sigma>\<^sub>c\<^sub>e \<Sigma>\<^sub>c\<^sub>e' rule: evalce.induct)
-  case (evce_lookup cd pc x env p v h vs sfs)
+proof (induction \<Sigma>\<^sub>c\<^sub>e \<Sigma>\<^sub>c\<^sub>e' rule: eval\<^sub>v.induct)
+  case (ev\<^sub>v_lookup cd pc x env p v h vs sfs)
   moreover hence "lookup (unstack_list env p) x = chain_lookup env p x" by auto
   ultimately show ?case by (simp add: unchain_stack_def)
 next
-  case (evce_apply cd pc h v2 p' pc' env v1 env' p'' vs p sfs)
-  from evce_apply have "chained_closures env h \<and> hcontains h v2" by simp
-  with evce_apply have "chained_closure env (CELam p' pc')" by (metis hlookup_all)
-  with evce_apply have "chain_structured h env \<and> chained_stack_pointer env p' \<and> 
+  case (ev\<^sub>v_apply cd pc h v2 p' pc' env v1 env' p'' vs p sfs)
+  from ev\<^sub>v_apply have "chained_closures env h \<and> hcontains h v2" by simp
+  with ev\<^sub>v_apply have "chained_closure env (Lam\<^sub>v p' pc')" by (metis hlookup_all)
+  with ev\<^sub>v_apply have "chain_structured h env \<and> chained_stack_pointer env p' \<and> 
     halloc env (v1, p') = (env', p'')" by auto
   hence X: "unstack_list env' (Suc p'') = v1 # unstack_list env p'" by (metis unfold_unstack_list)
-  from evce_apply have A: "unchain_heap h env' = unchain_heap h env" by auto
-  from evce_apply have B: "unstack_list env' p = unstack_list env p" by auto
-  from evce_apply have "unchain_stack env' sfs = unchain_stack env sfs" by auto 
-  with evce_apply X A B have "cd \<tturnstile> S\<^sub>h (unchain_heap h env) (v1 # v2 # vs) 
+  from ev\<^sub>v_apply have A: "unchain_heap h env' = unchain_heap h env" by auto
+  from ev\<^sub>v_apply have B: "unstack_list env' p = unstack_list env p" by auto
+  from ev\<^sub>v_apply have "unchain_stack env' sfs = unchain_stack env sfs" by auto 
+  with ev\<^sub>v_apply X A B have "cd \<tturnstile> S\<^sub>h (unchain_heap h env) (v1 # v2 # vs) 
     ((unstack_list env p, Suc pc) # unchain_stack env sfs) \<leadsto>\<^sub>h
       S\<^sub>h (unchain_heap h env') vs 
         ((unstack_list env' (Suc p''), pc') # (unstack_list env' p, pc) # unchain_stack env' sfs)" 
     by simp
   thus ?case by (simp add: unchain_stack_def)
 next
-  case (evce_jump cd pc h v2 p' pc' env v1 env' p'' vs p sfs)
-  from evce_jump have "chained_closures env h \<and> hcontains h v2" by simp
-  with evce_jump have "chained_closure env (CELam p' pc')" by (metis hlookup_all)
-  with evce_jump have "chain_structured h env \<and> chained_stack_pointer env p' \<and> 
+  case (ev\<^sub>v_jump cd pc h v2 p' pc' env v1 env' p'' vs p sfs)
+  from ev\<^sub>v_jump have "chained_closures env h \<and> hcontains h v2" by simp
+  with ev\<^sub>v_jump have "chained_closure env (Lam\<^sub>v p' pc')" by (metis hlookup_all)
+  with ev\<^sub>v_jump have "chain_structured h env \<and> chained_stack_pointer env p' \<and> 
     halloc env (v1, p') = (env', p'')" by auto
   hence X: "unstack_list env' (Suc p'') = v1 # unstack_list env p'" by (metis unfold_unstack_list)
-  from evce_jump have A: "unchain_heap h env' = unchain_heap h env" by auto
-  from evce_jump have "unchain_stack env' sfs = unchain_stack env sfs" by auto 
-  with evce_jump X A have "cd \<tturnstile> S\<^sub>h (unchain_heap h env) (v1 # v2 # vs) 
+  from ev\<^sub>v_jump have A: "unchain_heap h env' = unchain_heap h env" by auto
+  from ev\<^sub>v_jump have "unchain_stack env' sfs = unchain_stack env sfs" by auto 
+  with ev\<^sub>v_jump X A have "cd \<tturnstile> S\<^sub>h (unchain_heap h env) (v1 # v2 # vs) 
     ((unstack_list env p, Suc pc) # unchain_stack env sfs) \<leadsto>\<^sub>h
       S\<^sub>h (unchain_heap h env') vs 
         ((unstack_list env' (Suc p''), pc') # unchain_stack env' sfs)" by simp
@@ -423,11 +425,11 @@ proof -
   ultimately show "chained_closures env' h" by (metis heap_all_implication)
 qed
 
-lemma [simp]: "hlookup h v2 = CELam p' pc' \<Longrightarrow> chained_closures env h \<Longrightarrow> hcontains h v2 \<Longrightarrow> 
+lemma [simp]: "hlookup h v2 = Lam\<^sub>v p' pc' \<Longrightarrow> chained_closures env h \<Longrightarrow> hcontains h v2 \<Longrightarrow> 
   hcontains h v1 \<Longrightarrow> halloc env (v1, p') = (env', p'') \<Longrightarrow> chain_structured h env \<Longrightarrow> 
     chain_structured h env'"
 proof -
-  assume "chained_closures env h" and "hlookup h v2 = CELam p' pc'" and "hcontains h v2"
+  assume "chained_closures env h" and "hlookup h v2 = Lam\<^sub>v p' pc'" and "hcontains h v2"
   hence X: "chained_stack_pointer env p'" using hlookup_all by fastforce
   moreover assume A: "halloc env (v1, p') = (env', p'')" and "chain_structured h env" 
     and "hcontains h v1"
@@ -454,13 +456,13 @@ next
   ultimately show ?case by auto
 qed
 
-lemma [simp]: "cd \<tturnstile> \<Sigma>\<^sub>c\<^sub>e \<leadsto>\<^sub>c\<^sub>e \<Sigma>\<^sub>c\<^sub>e' \<Longrightarrow> chained_state \<Sigma>\<^sub>c\<^sub>e \<Longrightarrow> chained_state \<Sigma>\<^sub>c\<^sub>e'"
-proof (induction \<Sigma>\<^sub>c\<^sub>e \<Sigma>\<^sub>c\<^sub>e' rule: evalce.induct)
-  case (evce_lookup cd pc x env p v h vs sfs)
+lemma [simp]: "cd \<tturnstile> \<Sigma>\<^sub>c\<^sub>e \<leadsto>\<^sub>v \<Sigma>\<^sub>c\<^sub>e' \<Longrightarrow> chained_state \<Sigma>\<^sub>c\<^sub>e \<Longrightarrow> chained_state \<Sigma>\<^sub>c\<^sub>e'"
+proof (induction \<Sigma>\<^sub>c\<^sub>e \<Sigma>\<^sub>c\<^sub>e' rule: eval\<^sub>v.induct)
+  case (ev\<^sub>v_lookup cd pc x env p v h vs sfs)
   thus ?case by (cases p) auto
 qed auto
 
-lemma [simp]: "iter (\<tturnstile> cd \<leadsto>\<^sub>c\<^sub>e) \<Sigma>\<^sub>c\<^sub>e \<Sigma>\<^sub>c\<^sub>e' \<Longrightarrow> chained_state \<Sigma>\<^sub>c\<^sub>e \<Longrightarrow> 
+lemma [simp]: "iter (\<tturnstile> cd \<leadsto>\<^sub>v) \<Sigma>\<^sub>c\<^sub>e \<Sigma>\<^sub>c\<^sub>e' \<Longrightarrow> chained_state \<Sigma>\<^sub>c\<^sub>e \<Longrightarrow> 
   iter (\<tturnstile> cd \<leadsto>\<^sub>h) (unchain_state \<Sigma>\<^sub>c\<^sub>e) (unchain_state \<Sigma>\<^sub>c\<^sub>e')"
 proof (induction \<Sigma>\<^sub>c\<^sub>e \<Sigma>\<^sub>c\<^sub>e' rule: iter.induct)
   case (iter_step \<Sigma>\<^sub>c\<^sub>e \<Sigma>\<^sub>c\<^sub>e' \<Sigma>\<^sub>c\<^sub>e'')
@@ -470,17 +472,17 @@ proof (induction \<Sigma>\<^sub>c\<^sub>e \<Sigma>\<^sub>c\<^sub>e' rule: iter.i
 qed simp_all
 
 lemma [simp]: "iter (\<tturnstile> cd \<leadsto>\<^sub>h) (unchain_state \<Sigma>\<^sub>c\<^sub>e) \<Sigma>\<^sub>h \<Longrightarrow> chained_state \<Sigma>\<^sub>c\<^sub>e \<Longrightarrow> 
-  \<exists>\<Sigma>\<^sub>c\<^sub>e'. iter (\<tturnstile> cd \<leadsto>\<^sub>c\<^sub>e) \<Sigma>\<^sub>c\<^sub>e \<Sigma>\<^sub>c\<^sub>e' \<and> \<Sigma>\<^sub>h = unchain_state \<Sigma>\<^sub>c\<^sub>e'"
+  \<exists>\<Sigma>\<^sub>c\<^sub>e'. iter (\<tturnstile> cd \<leadsto>\<^sub>v) \<Sigma>\<^sub>c\<^sub>e \<Sigma>\<^sub>c\<^sub>e' \<and> \<Sigma>\<^sub>h = unchain_state \<Sigma>\<^sub>c\<^sub>e'"
 proof (induction "unchain_state \<Sigma>\<^sub>c\<^sub>e" \<Sigma>\<^sub>h arbitrary: \<Sigma>\<^sub>c\<^sub>e rule: iter.induct)
   case (iter_step \<Sigma>\<^sub>h' \<Sigma>\<^sub>h'')
-  then obtain \<Sigma>\<^sub>c\<^sub>e' where "(cd \<tturnstile> \<Sigma>\<^sub>c\<^sub>e \<leadsto>\<^sub>c\<^sub>e \<Sigma>\<^sub>c\<^sub>e') \<and> \<Sigma>\<^sub>h' = unchain_state \<Sigma>\<^sub>c\<^sub>e'" by fastforce
-  moreover with iter_step obtain \<Sigma>\<^sub>c\<^sub>e'' where "iter (\<tturnstile> cd \<leadsto>\<^sub>c\<^sub>e) \<Sigma>\<^sub>c\<^sub>e' \<Sigma>\<^sub>c\<^sub>e'' \<and> 
+  then obtain \<Sigma>\<^sub>c\<^sub>e' where "(cd \<tturnstile> \<Sigma>\<^sub>c\<^sub>e \<leadsto>\<^sub>v \<Sigma>\<^sub>c\<^sub>e') \<and> \<Sigma>\<^sub>h' = unchain_state \<Sigma>\<^sub>c\<^sub>e'" by fastforce
+  moreover with iter_step obtain \<Sigma>\<^sub>c\<^sub>e'' where "iter (\<tturnstile> cd \<leadsto>\<^sub>v) \<Sigma>\<^sub>c\<^sub>e' \<Sigma>\<^sub>c\<^sub>e'' \<and> 
     \<Sigma>\<^sub>h'' = unchain_state \<Sigma>\<^sub>c\<^sub>e''" by fastforce
-  ultimately have "iter (\<tturnstile> cd \<leadsto>\<^sub>c\<^sub>e) \<Sigma>\<^sub>c\<^sub>e \<Sigma>\<^sub>c\<^sub>e'' \<and> \<Sigma>\<^sub>h'' = unchain_state \<Sigma>\<^sub>c\<^sub>e''" by fastforce
+  ultimately have "iter (\<tturnstile> cd \<leadsto>\<^sub>v) \<Sigma>\<^sub>c\<^sub>e \<Sigma>\<^sub>c\<^sub>e'' \<and> \<Sigma>\<^sub>h'' = unchain_state \<Sigma>\<^sub>c\<^sub>e''" by fastforce
   then show ?case by fastforce
 qed force+
 
-lemma preserve_chained [simp]: "iter (\<tturnstile> cd \<leadsto>\<^sub>c\<^sub>e) \<Sigma>\<^sub>c\<^sub>e \<Sigma>\<^sub>c\<^sub>e' \<Longrightarrow> chained_state \<Sigma>\<^sub>c\<^sub>e \<Longrightarrow> 
+lemma preserve_chained [simp]: "iter (\<tturnstile> cd \<leadsto>\<^sub>v) \<Sigma>\<^sub>c\<^sub>e \<Sigma>\<^sub>c\<^sub>e' \<Longrightarrow> chained_state \<Sigma>\<^sub>c\<^sub>e \<Longrightarrow> 
     chained_state \<Sigma>\<^sub>c\<^sub>e'"
   by (induction \<Sigma>\<^sub>c\<^sub>e \<Sigma>\<^sub>c\<^sub>e' rule: iter.induct) simp_all
 
