10FlatMemory/MemoryFlattening.thy
@@ -2,15 +2,15 @@ theory MemoryFlattening
   imports FlatMemory "../08HeapMemory/HeapConversion" "../09ChainedEnvironment/Chaining"
 begin
 
-primrec flatten_closure :: "ceclosure \<Rightarrow> nat list" where
-  "flatten_closure (CEConst k) = [1, k, 0]"
-| "flatten_closure (CELam p pc) = [0, 2 * p, pc]"
+primrec flatten_closure :: "closure\<^sub>v \<Rightarrow> nat list" where
+  "flatten_closure (Const\<^sub>v k) = [1, k, 0]"
+| "flatten_closure (Lam\<^sub>v p pc) = [0, 2 * p, pc]"
 
-primrec flatten_closure' :: "ceclosure \<Rightarrow> ceclosure" where
-  "flatten_closure' (CEConst k) = CEConst k"
-| "flatten_closure' (CELam p pc) = CELam (2 * p) pc"
+primrec flatten_closure' :: "closure\<^sub>v \<Rightarrow> closure\<^sub>v" where
+  "flatten_closure' (Const\<^sub>v k) = Const\<^sub>v k"
+| "flatten_closure' (Lam\<^sub>v p pc) = Lam\<^sub>v (2 * p) pc"
 
-abbreviation flatten_values :: "ceclosure heap \<Rightarrow> nat heap" where
+abbreviation flatten_values :: "closure\<^sub>v heap \<Rightarrow> nat heap" where
   "flatten_values h \<equiv> hsplay flatten_closure h"
 
 primrec flatten_env :: "(ptr \<times> ptr) \<Rightarrow> ptr list" where
@@ -28,21 +28,21 @@ primrec flatten_frame :: "(ptr \<times> nat) \<Rightarrow> nat list" where
 abbreviation flatten_stack :: "(ptr \<times> nat) list \<Rightarrow> nat list" where
   "flatten_stack sfs \<equiv> concat (map flatten_frame sfs)"
 
-primrec flatten :: "chained_state \<Rightarrow> flat_state" where
-  "flatten (CES h env vs sfs) = 
+primrec flatten :: "state\<^sub>v \<Rightarrow> flat_state" where
+  "flatten (S\<^sub>v h env vs sfs) = 
       FS (flatten_values h) (flatten_environment env) (flatten_vals vs) (flatten_stack sfs)"
 
 lemma [simp]: "length (flatten_closure c) = 3"
   by (induction c) simp_all
 
-lemma [simp]: "flatten_closure c ! 0 = (case c of CELam _ _ \<Rightarrow> 0 | CEConst _ \<Rightarrow> 1)"
-  by (simp split: ceclosure.splits)
+lemma [simp]: "flatten_closure c ! 0 = (case c of Lam\<^sub>v _ _ \<Rightarrow> 0 | Const\<^sub>v _ \<Rightarrow> 1)"
+  by (simp split: closure\<^sub>v.splits)
 
-lemma flatten_c1 [simp]: "flatten_closure c ! 1 = (case c of CEConst k \<Rightarrow> k | CELam p _ \<Rightarrow> 2 * p)"
-  by (simp split: ceclosure.splits)
+lemma flatten_c1 [simp]: "flatten_closure c ! 1 = (case c of Const\<^sub>v k \<Rightarrow> k | Lam\<^sub>v p _ \<Rightarrow> 2 * p)"
+  by (simp split: closure\<^sub>v.splits)
 
-lemma flatten_c2 [simp]: "flatten_closure c ! 2 = (case c of CEConst k \<Rightarrow> 0 | CELam _ pc \<Rightarrow> pc)"
-  by (simp split: ceclosure.splits)
+lemma flatten_c2 [simp]: "flatten_closure c ! 2 = (case c of Const\<^sub>v k \<Rightarrow> 0 | Lam\<^sub>v _ pc \<Rightarrow> pc)"
+  by (simp split: closure\<^sub>v.splits)
 
 lemma [simp]: "hcontains h v \<Longrightarrow> 
   get_closure (flatten_values h) (3 * v) = flatten_closure' (hlookup h v)"
@@ -51,22 +51,22 @@ proof -
   hence H: "\<And>k g. (\<And>a. flatten_closure a ! k = g a) \<Longrightarrow>
     k < 3 \<Longrightarrow> hlookup (hsplay flatten_closure h) (k + 3 * v) = g (hlookup h v)" by simp
   hence "hlookup (hsplay flatten_closure h) (3 * v) = 
-    (case hlookup h v of CELam _ _ \<Rightarrow> 0 | CEConst _ \<Rightarrow> 1)" by force
+    (case hlookup h v of Lam\<^sub>v _ _ \<Rightarrow> 0 | Const\<^sub>v _ \<Rightarrow> 1)" by force
   moreover from H have "hlookup (hsplay flatten_closure h) (Suc (3 * v)) = 
-    (case hlookup h v of CELam p _ \<Rightarrow> 2 * p | CEConst k \<Rightarrow> k)"
+    (case hlookup h v of Lam\<^sub>v p _ \<Rightarrow> 2 * p | Const\<^sub>v k \<Rightarrow> k)"
       by (metis flatten_c1 one_less_numeral_iff plus_1_eq_Suc semiring_norm(77))
   moreover from H have "hlookup (hsplay flatten_closure h) (Suc (Suc (3 * v))) = 
-    (case hlookup h v of CELam _ pc \<Rightarrow> pc | CEConst k \<Rightarrow> 0)"
+    (case hlookup h v of Lam\<^sub>v _ pc \<Rightarrow> pc | Const\<^sub>v k \<Rightarrow> 0)"
       by (metis flatten_c2 add.left_neutral add_2_eq_Suc' add_Suc eval_nat_numeral(3) lessI)
-  ultimately show ?thesis by (simp split: ceclosure.splits)
+  ultimately show ?thesis by (simp split: closure\<^sub>v.splits)
 qed
 
-lemma [dest]: "hcontains h v \<Longrightarrow> get_closure (flatten_values h) (3 * v) = CEConst k \<Longrightarrow> 
-    hlookup h v = CEConst k"
+lemma [dest]: "hcontains h v \<Longrightarrow> get_closure (flatten_values h) (3 * v) = Const\<^sub>v k \<Longrightarrow> 
+    hlookup h v = Const\<^sub>v k"
   by (cases "hlookup h v") (simp_all del: get_closure.simps)
 
-lemma [dest]: "hcontains h v \<Longrightarrow> get_closure (flatten_values h) (3 * v) = CELam p pc \<Longrightarrow> 
-    \<exists>p'. hlookup h v = CELam p' pc \<and> p = 2 * p'"
+lemma [dest]: "hcontains h v \<Longrightarrow> get_closure (flatten_values h) (3 * v) = Lam\<^sub>v p pc \<Longrightarrow> 
+    \<exists>p'. hlookup h v = Lam\<^sub>v p' pc \<and> p = 2 * p'"
   by (cases "hlookup h v") (simp_all del: get_closure.simps)
 
 lemma [simp]: "length (flatten_env e) = 2"
@@ -109,7 +109,7 @@ lemma flatten_halloc [simp]: "halloc h c = (h', v) \<Longrightarrow>
 lemma flatten_lt_3: "hcontains h x \<Longrightarrow> flatten_values h = H h' hp \<Longrightarrow> Suc (3 * x) < hp"
   by simp
 
-lemma [dest]: "FS h env vs sfs = flatten \<Sigma>\<^sub>c\<^sub>e \<Longrightarrow> \<exists>h\<^sub>c\<^sub>e env\<^sub>c\<^sub>e vs\<^sub>c\<^sub>e sfs\<^sub>c\<^sub>e. \<Sigma>\<^sub>c\<^sub>e = CES h\<^sub>c\<^sub>e env\<^sub>c\<^sub>e vs\<^sub>c\<^sub>e sfs\<^sub>c\<^sub>e \<and> 
+lemma [dest]: "FS h env vs sfs = flatten \<Sigma>\<^sub>c\<^sub>e \<Longrightarrow> \<exists>h\<^sub>c\<^sub>e env\<^sub>c\<^sub>e vs\<^sub>c\<^sub>e sfs\<^sub>c\<^sub>e. \<Sigma>\<^sub>c\<^sub>e = S\<^sub>v h\<^sub>c\<^sub>e env\<^sub>c\<^sub>e vs\<^sub>c\<^sub>e sfs\<^sub>c\<^sub>e \<and> 
   h = flatten_values h\<^sub>c\<^sub>e \<and> env = flatten_environment env\<^sub>c\<^sub>e \<and> vs = flatten_vals vs\<^sub>c\<^sub>e \<and> 
     sfs = flatten_stack sfs\<^sub>c\<^sub>e"
   by (induction \<Sigma>\<^sub>c\<^sub>e) simp_all
@@ -140,108 +140,108 @@ proof -
 qed
 
 theorem correctf: "cd \<tturnstile> flatten \<Sigma>\<^sub>c\<^sub>e \<leadsto>\<^sub>f \<Sigma>\<^sub>f' \<Longrightarrow> chained_state \<Sigma>\<^sub>c\<^sub>e \<Longrightarrow> 
-  \<exists>\<Sigma>\<^sub>c\<^sub>e'. (cd \<tturnstile> \<Sigma>\<^sub>c\<^sub>e \<leadsto>\<^sub>c\<^sub>e \<Sigma>\<^sub>c\<^sub>e') \<and> flatten \<Sigma>\<^sub>c\<^sub>e' = \<Sigma>\<^sub>f'" 
+  \<exists>\<Sigma>\<^sub>c\<^sub>e'. (cd \<tturnstile> \<Sigma>\<^sub>c\<^sub>e \<leadsto>\<^sub>v \<Sigma>\<^sub>c\<^sub>e') \<and> flatten \<Sigma>\<^sub>c\<^sub>e' = \<Sigma>\<^sub>f'" 
 proof (induction "flatten \<Sigma>\<^sub>c\<^sub>e" \<Sigma>\<^sub>f' rule: evalf.induct)
   case (evf_lookup cd pc x env p v h vs sfs)
-  then obtain h\<^sub>c\<^sub>e env\<^sub>c\<^sub>e vs\<^sub>c\<^sub>e p\<^sub>c\<^sub>e sfs\<^sub>c\<^sub>e where S: "\<Sigma>\<^sub>c\<^sub>e = CES h\<^sub>c\<^sub>e env\<^sub>c\<^sub>e vs\<^sub>c\<^sub>e ((p\<^sub>c\<^sub>e, Suc pc) # sfs\<^sub>c\<^sub>e) \<and> 
+  then obtain h\<^sub>c\<^sub>e env\<^sub>c\<^sub>e vs\<^sub>c\<^sub>e p\<^sub>c\<^sub>e sfs\<^sub>c\<^sub>e where S: "\<Sigma>\<^sub>c\<^sub>e = S\<^sub>v h\<^sub>c\<^sub>e env\<^sub>c\<^sub>e vs\<^sub>c\<^sub>e ((p\<^sub>c\<^sub>e, Suc pc) # sfs\<^sub>c\<^sub>e) \<and> 
     h = flatten_values h\<^sub>c\<^sub>e \<and> env = flatten_environment env\<^sub>c\<^sub>e \<and> vs = flatten_vals vs\<^sub>c\<^sub>e \<and> 
       sfs = flatten_stack sfs\<^sub>c\<^sub>e \<and> p = 2 * p\<^sub>c\<^sub>e" by fastforce
   with evf_lookup obtain v\<^sub>c\<^sub>e where V: "chain_lookup env\<^sub>c\<^sub>e p\<^sub>c\<^sub>e x = Some v\<^sub>c\<^sub>e \<and> v = 3 * v\<^sub>c\<^sub>e" by fastforce
-  with S have X: "flatten (CES h\<^sub>c\<^sub>e env\<^sub>c\<^sub>e (v\<^sub>c\<^sub>e # vs\<^sub>c\<^sub>e) ((p\<^sub>c\<^sub>e, pc) # sfs\<^sub>c\<^sub>e)) = 
+  with S have X: "flatten (S\<^sub>v h\<^sub>c\<^sub>e env\<^sub>c\<^sub>e (v\<^sub>c\<^sub>e # vs\<^sub>c\<^sub>e) ((p\<^sub>c\<^sub>e, pc) # sfs\<^sub>c\<^sub>e)) = 
     FS h env (v # vs) (pc # p # sfs)" by simp
-  from evf_lookup V have "cd \<tturnstile> CES h\<^sub>c\<^sub>e env\<^sub>c\<^sub>e vs\<^sub>c\<^sub>e ((p\<^sub>c\<^sub>e, Suc pc) # sfs\<^sub>c\<^sub>e) \<leadsto>\<^sub>c\<^sub>e 
-    CES h\<^sub>c\<^sub>e env\<^sub>c\<^sub>e (v\<^sub>c\<^sub>e # vs\<^sub>c\<^sub>e) ((p\<^sub>c\<^sub>e, pc) # sfs\<^sub>c\<^sub>e)" by simp
+  from evf_lookup V have "cd \<tturnstile> S\<^sub>v h\<^sub>c\<^sub>e env\<^sub>c\<^sub>e vs\<^sub>c\<^sub>e ((p\<^sub>c\<^sub>e, Suc pc) # sfs\<^sub>c\<^sub>e) \<leadsto>\<^sub>v 
+    S\<^sub>v h\<^sub>c\<^sub>e env\<^sub>c\<^sub>e (v\<^sub>c\<^sub>e # vs\<^sub>c\<^sub>e) ((p\<^sub>c\<^sub>e, pc) # sfs\<^sub>c\<^sub>e)" by simp
   with S X show ?case by blast
 next
   case (evf_pushcon cd pc k h h' v env vs p sfs)
-  then obtain h\<^sub>c\<^sub>e env\<^sub>c\<^sub>e vs\<^sub>c\<^sub>e p\<^sub>c\<^sub>e sfs\<^sub>c\<^sub>e where S: "\<Sigma>\<^sub>c\<^sub>e = CES h\<^sub>c\<^sub>e env\<^sub>c\<^sub>e vs\<^sub>c\<^sub>e ((p\<^sub>c\<^sub>e, Suc pc) # sfs\<^sub>c\<^sub>e) \<and> 
+  then obtain h\<^sub>c\<^sub>e env\<^sub>c\<^sub>e vs\<^sub>c\<^sub>e p\<^sub>c\<^sub>e sfs\<^sub>c\<^sub>e where S: "\<Sigma>\<^sub>c\<^sub>e = S\<^sub>v h\<^sub>c\<^sub>e env\<^sub>c\<^sub>e vs\<^sub>c\<^sub>e ((p\<^sub>c\<^sub>e, Suc pc) # sfs\<^sub>c\<^sub>e) \<and> 
     h = flatten_values h\<^sub>c\<^sub>e \<and> env = flatten_environment env\<^sub>c\<^sub>e \<and> vs = flatten_vals vs\<^sub>c\<^sub>e \<and> 
       sfs = flatten_stack sfs\<^sub>c\<^sub>e \<and> p = 2 * p\<^sub>c\<^sub>e" by fastforce
-  with evf_pushcon have "halloc_list (hsplay flatten_closure h\<^sub>c\<^sub>e) (flatten_closure (CEConst k)) = 
+  with evf_pushcon have "halloc_list (hsplay flatten_closure h\<^sub>c\<^sub>e) (flatten_closure (Const\<^sub>v k)) = 
     (h', v)" by simp
   then obtain h\<^sub>c\<^sub>e' v\<^sub>c\<^sub>e where H: "h' = hsplay flatten_closure h\<^sub>c\<^sub>e' \<and> v = 3 * v\<^sub>c\<^sub>e \<and> 
-    halloc h\<^sub>c\<^sub>e (CEConst k) = (h\<^sub>c\<^sub>e', v\<^sub>c\<^sub>e)" by fastforce
-  with S have X: "flatten (CES h\<^sub>c\<^sub>e' env\<^sub>c\<^sub>e (v\<^sub>c\<^sub>e # vs\<^sub>c\<^sub>e) ((p\<^sub>c\<^sub>e, pc) # sfs\<^sub>c\<^sub>e)) = 
+    halloc h\<^sub>c\<^sub>e (Const\<^sub>v k) = (h\<^sub>c\<^sub>e', v\<^sub>c\<^sub>e)" by fastforce
+  with S have X: "flatten (S\<^sub>v h\<^sub>c\<^sub>e' env\<^sub>c\<^sub>e (v\<^sub>c\<^sub>e # vs\<^sub>c\<^sub>e) ((p\<^sub>c\<^sub>e, pc) # sfs\<^sub>c\<^sub>e)) = 
     FS h' env (v # vs) (pc # p # sfs)" by simp
-  from evf_pushcon H have "cd \<tturnstile> CES h\<^sub>c\<^sub>e env\<^sub>c\<^sub>e vs\<^sub>c\<^sub>e ((p\<^sub>c\<^sub>e, Suc pc) # sfs\<^sub>c\<^sub>e) \<leadsto>\<^sub>c\<^sub>e 
-    CES h\<^sub>c\<^sub>e' env\<^sub>c\<^sub>e (v\<^sub>c\<^sub>e # vs\<^sub>c\<^sub>e) ((p\<^sub>c\<^sub>e, pc) # sfs\<^sub>c\<^sub>e)" by simp
+  from evf_pushcon H have "cd \<tturnstile> S\<^sub>v h\<^sub>c\<^sub>e env\<^sub>c\<^sub>e vs\<^sub>c\<^sub>e ((p\<^sub>c\<^sub>e, Suc pc) # sfs\<^sub>c\<^sub>e) \<leadsto>\<^sub>v 
+    S\<^sub>v h\<^sub>c\<^sub>e' env\<^sub>c\<^sub>e (v\<^sub>c\<^sub>e # vs\<^sub>c\<^sub>e) ((p\<^sub>c\<^sub>e, pc) # sfs\<^sub>c\<^sub>e)" by simp
   with S X show ?case by blast
 next
   case (evf_pushlam cd pc pc' h p h' v env vs sfs)
-  then obtain h\<^sub>c\<^sub>e env\<^sub>c\<^sub>e vs\<^sub>c\<^sub>e p\<^sub>c\<^sub>e sfs\<^sub>c\<^sub>e where S: "\<Sigma>\<^sub>c\<^sub>e = CES h\<^sub>c\<^sub>e env\<^sub>c\<^sub>e vs\<^sub>c\<^sub>e ((p\<^sub>c\<^sub>e, Suc pc) # sfs\<^sub>c\<^sub>e) \<and> 
+  then obtain h\<^sub>c\<^sub>e env\<^sub>c\<^sub>e vs\<^sub>c\<^sub>e p\<^sub>c\<^sub>e sfs\<^sub>c\<^sub>e where S: "\<Sigma>\<^sub>c\<^sub>e = S\<^sub>v h\<^sub>c\<^sub>e env\<^sub>c\<^sub>e vs\<^sub>c\<^sub>e ((p\<^sub>c\<^sub>e, Suc pc) # sfs\<^sub>c\<^sub>e) \<and> 
     h = flatten_values h\<^sub>c\<^sub>e \<and> env = flatten_environment env\<^sub>c\<^sub>e \<and> vs = flatten_vals vs\<^sub>c\<^sub>e \<and> 
       sfs = flatten_stack sfs\<^sub>c\<^sub>e \<and> p = 2 * p\<^sub>c\<^sub>e" by fastforce
-  with evf_pushlam have "halloc_list (hsplay flatten_closure h\<^sub>c\<^sub>e) (flatten_closure (CELam p\<^sub>c\<^sub>e pc')) = 
+  with evf_pushlam have "halloc_list (hsplay flatten_closure h\<^sub>c\<^sub>e) (flatten_closure (Lam\<^sub>v p\<^sub>c\<^sub>e pc')) = 
     (h', v)" by simp
   then obtain h\<^sub>c\<^sub>e' v\<^sub>c\<^sub>e where H: "h' = hsplay flatten_closure h\<^sub>c\<^sub>e' \<and> v = 3 * v\<^sub>c\<^sub>e \<and> 
-    halloc h\<^sub>c\<^sub>e (CELam p\<^sub>c\<^sub>e pc') = (h\<^sub>c\<^sub>e', v\<^sub>c\<^sub>e)" by fastforce
-  with S have X: "flatten (CES h\<^sub>c\<^sub>e' env\<^sub>c\<^sub>e (v\<^sub>c\<^sub>e # vs\<^sub>c\<^sub>e) ((p\<^sub>c\<^sub>e, pc) # sfs\<^sub>c\<^sub>e)) = 
+    halloc h\<^sub>c\<^sub>e (Lam\<^sub>v p\<^sub>c\<^sub>e pc') = (h\<^sub>c\<^sub>e', v\<^sub>c\<^sub>e)" by fastforce
+  with S have X: "flatten (S\<^sub>v h\<^sub>c\<^sub>e' env\<^sub>c\<^sub>e (v\<^sub>c\<^sub>e # vs\<^sub>c\<^sub>e) ((p\<^sub>c\<^sub>e, pc) # sfs\<^sub>c\<^sub>e)) = 
     FS h' env (v # vs) (pc # p # sfs)" by simp
-  from evf_pushlam S H have "cd \<tturnstile> CES h\<^sub>c\<^sub>e env\<^sub>c\<^sub>e vs\<^sub>c\<^sub>e ((p\<^sub>c\<^sub>e, Suc pc) # sfs\<^sub>c\<^sub>e) \<leadsto>\<^sub>c\<^sub>e 
-    CES h\<^sub>c\<^sub>e' env\<^sub>c\<^sub>e (v\<^sub>c\<^sub>e # vs\<^sub>c\<^sub>e) ((p\<^sub>c\<^sub>e, pc) # sfs\<^sub>c\<^sub>e)" by simp
+  from evf_pushlam S H have "cd \<tturnstile> S\<^sub>v h\<^sub>c\<^sub>e env\<^sub>c\<^sub>e vs\<^sub>c\<^sub>e ((p\<^sub>c\<^sub>e, Suc pc) # sfs\<^sub>c\<^sub>e) \<leadsto>\<^sub>v 
+    S\<^sub>v h\<^sub>c\<^sub>e' env\<^sub>c\<^sub>e (v\<^sub>c\<^sub>e # vs\<^sub>c\<^sub>e) ((p\<^sub>c\<^sub>e, pc) # sfs\<^sub>c\<^sub>e)" by simp
   with S X show ?case by blast
 next
   case (evf_apply cd pc h v2 p' pc' env v1 env' p2 vs p sfs)
   then obtain h\<^sub>c\<^sub>e env\<^sub>c\<^sub>e v1\<^sub>c\<^sub>e v2\<^sub>c\<^sub>e vs\<^sub>c\<^sub>e p\<^sub>c\<^sub>e sfs\<^sub>c\<^sub>e where S: "
-    \<Sigma>\<^sub>c\<^sub>e = CES h\<^sub>c\<^sub>e env\<^sub>c\<^sub>e (v1\<^sub>c\<^sub>e # v2\<^sub>c\<^sub>e # vs\<^sub>c\<^sub>e) ((p\<^sub>c\<^sub>e, Suc pc) # sfs\<^sub>c\<^sub>e) \<and> h = flatten_values h\<^sub>c\<^sub>e \<and> 
+    \<Sigma>\<^sub>c\<^sub>e = S\<^sub>v h\<^sub>c\<^sub>e env\<^sub>c\<^sub>e (v1\<^sub>c\<^sub>e # v2\<^sub>c\<^sub>e # vs\<^sub>c\<^sub>e) ((p\<^sub>c\<^sub>e, Suc pc) # sfs\<^sub>c\<^sub>e) \<and> h = flatten_values h\<^sub>c\<^sub>e \<and> 
       env = flatten_environment env\<^sub>c\<^sub>e \<and> v1 = 3 * v1\<^sub>c\<^sub>e \<and> v2 = 3 * v2\<^sub>c\<^sub>e \<and> vs = flatten_vals vs\<^sub>c\<^sub>e \<and> 
         sfs = flatten_stack sfs\<^sub>c\<^sub>e \<and> p = 2 * p\<^sub>c\<^sub>e" by fastforce
-  with evf_apply have "get_closure (flatten_values h\<^sub>c\<^sub>e) (3 * v2\<^sub>c\<^sub>e) = CELam p' pc'" by simp
+  with evf_apply have "get_closure (flatten_values h\<^sub>c\<^sub>e) (3 * v2\<^sub>c\<^sub>e) = Lam\<^sub>v p' pc'" by simp
   moreover from evf_apply S have "hcontains h\<^sub>c\<^sub>e v2\<^sub>c\<^sub>e" by simp
-  ultimately obtain p\<^sub>c\<^sub>e' where P: "hlookup h\<^sub>c\<^sub>e v2\<^sub>c\<^sub>e = CELam p\<^sub>c\<^sub>e' pc' \<and> p' = 2 * p\<^sub>c\<^sub>e'" by blast
+  ultimately obtain p\<^sub>c\<^sub>e' where P: "hlookup h\<^sub>c\<^sub>e v2\<^sub>c\<^sub>e = Lam\<^sub>v p\<^sub>c\<^sub>e' pc' \<and> p' = 2 * p\<^sub>c\<^sub>e'" by blast
   obtain env\<^sub>c\<^sub>e' p2\<^sub>c\<^sub>e where E: "halloc env\<^sub>c\<^sub>e (v1\<^sub>c\<^sub>e, p\<^sub>c\<^sub>e') = (env\<^sub>c\<^sub>e', p2\<^sub>c\<^sub>e)" by fastforce
-  with evf_apply S P have X: "flatten (CES h\<^sub>c\<^sub>e env\<^sub>c\<^sub>e' vs\<^sub>c\<^sub>e ((Suc p2\<^sub>c\<^sub>e, pc') # (p\<^sub>c\<^sub>e, pc) # sfs\<^sub>c\<^sub>e)) = 
+  with evf_apply S P have X: "flatten (S\<^sub>v h\<^sub>c\<^sub>e env\<^sub>c\<^sub>e' vs\<^sub>c\<^sub>e ((Suc p2\<^sub>c\<^sub>e, pc') # (p\<^sub>c\<^sub>e, pc) # sfs\<^sub>c\<^sub>e)) = 
     FS h env' vs (pc' # Suc (Suc p2) # pc # p # sfs)" by simp
-  from evf_apply P E have "cd \<tturnstile> CES h\<^sub>c\<^sub>e env\<^sub>c\<^sub>e (v1\<^sub>c\<^sub>e # v2\<^sub>c\<^sub>e # vs\<^sub>c\<^sub>e) ((p\<^sub>c\<^sub>e, Suc pc) # sfs\<^sub>c\<^sub>e) \<leadsto>\<^sub>c\<^sub>e 
-    CES h\<^sub>c\<^sub>e env\<^sub>c\<^sub>e' vs\<^sub>c\<^sub>e ((Suc p2\<^sub>c\<^sub>e, pc') # (p\<^sub>c\<^sub>e, pc) # sfs\<^sub>c\<^sub>e)" by simp
+  from evf_apply P E have "cd \<tturnstile> S\<^sub>v h\<^sub>c\<^sub>e env\<^sub>c\<^sub>e (v1\<^sub>c\<^sub>e # v2\<^sub>c\<^sub>e # vs\<^sub>c\<^sub>e) ((p\<^sub>c\<^sub>e, Suc pc) # sfs\<^sub>c\<^sub>e) \<leadsto>\<^sub>v 
+    S\<^sub>v h\<^sub>c\<^sub>e env\<^sub>c\<^sub>e' vs\<^sub>c\<^sub>e ((Suc p2\<^sub>c\<^sub>e, pc') # (p\<^sub>c\<^sub>e, pc) # sfs\<^sub>c\<^sub>e)" by simp
   with S X show ?case by blast
 next
   case (evf_return cd pc h env vs p sfs)
-  then obtain h\<^sub>c\<^sub>e env\<^sub>c\<^sub>e vs\<^sub>c\<^sub>e p\<^sub>c\<^sub>e sfs\<^sub>c\<^sub>e where S: "\<Sigma>\<^sub>c\<^sub>e = CES h\<^sub>c\<^sub>e env\<^sub>c\<^sub>e vs\<^sub>c\<^sub>e ((p\<^sub>c\<^sub>e, Suc pc) # sfs\<^sub>c\<^sub>e) \<and> 
+  then obtain h\<^sub>c\<^sub>e env\<^sub>c\<^sub>e vs\<^sub>c\<^sub>e p\<^sub>c\<^sub>e sfs\<^sub>c\<^sub>e where S: "\<Sigma>\<^sub>c\<^sub>e = S\<^sub>v h\<^sub>c\<^sub>e env\<^sub>c\<^sub>e vs\<^sub>c\<^sub>e ((p\<^sub>c\<^sub>e, Suc pc) # sfs\<^sub>c\<^sub>e) \<and> 
     h = flatten_values h\<^sub>c\<^sub>e \<and> env = flatten_environment env\<^sub>c\<^sub>e \<and> vs = flatten_vals vs\<^sub>c\<^sub>e \<and> 
       sfs = flatten_stack sfs\<^sub>c\<^sub>e \<and> p = 2 * p\<^sub>c\<^sub>e" by fastforce
-  hence X: "flatten (CES h\<^sub>c\<^sub>e env\<^sub>c\<^sub>e vs\<^sub>c\<^sub>e sfs\<^sub>c\<^sub>e) = FS h env vs sfs" by simp
-  from evf_return have "cd \<tturnstile> CES h\<^sub>c\<^sub>e env\<^sub>c\<^sub>e vs\<^sub>c\<^sub>e ((p\<^sub>c\<^sub>e, Suc pc) # sfs\<^sub>c\<^sub>e) \<leadsto>\<^sub>c\<^sub>e 
-    CES h\<^sub>c\<^sub>e env\<^sub>c\<^sub>e vs\<^sub>c\<^sub>e sfs\<^sub>c\<^sub>e" by simp
+  hence X: "flatten (S\<^sub>v h\<^sub>c\<^sub>e env\<^sub>c\<^sub>e vs\<^sub>c\<^sub>e sfs\<^sub>c\<^sub>e) = FS h env vs sfs" by simp
+  from evf_return have "cd \<tturnstile> S\<^sub>v h\<^sub>c\<^sub>e env\<^sub>c\<^sub>e vs\<^sub>c\<^sub>e ((p\<^sub>c\<^sub>e, Suc pc) # sfs\<^sub>c\<^sub>e) \<leadsto>\<^sub>v 
+    S\<^sub>v h\<^sub>c\<^sub>e env\<^sub>c\<^sub>e vs\<^sub>c\<^sub>e sfs\<^sub>c\<^sub>e" by simp
   with S X show ?case by blast
 next
   case (evf_jump cd pc h v2 p' pc' env v1 env' p2 vs p sfs)
   then obtain h\<^sub>c\<^sub>e env\<^sub>c\<^sub>e v1\<^sub>c\<^sub>e v2\<^sub>c\<^sub>e vs\<^sub>c\<^sub>e p\<^sub>c\<^sub>e sfs\<^sub>c\<^sub>e where S: "
-    \<Sigma>\<^sub>c\<^sub>e = CES h\<^sub>c\<^sub>e env\<^sub>c\<^sub>e (v1\<^sub>c\<^sub>e # v2\<^sub>c\<^sub>e # vs\<^sub>c\<^sub>e) ((p\<^sub>c\<^sub>e, Suc pc) # sfs\<^sub>c\<^sub>e) \<and> h = flatten_values h\<^sub>c\<^sub>e \<and> 
+    \<Sigma>\<^sub>c\<^sub>e = S\<^sub>v h\<^sub>c\<^sub>e env\<^sub>c\<^sub>e (v1\<^sub>c\<^sub>e # v2\<^sub>c\<^sub>e # vs\<^sub>c\<^sub>e) ((p\<^sub>c\<^sub>e, Suc pc) # sfs\<^sub>c\<^sub>e) \<and> h = flatten_values h\<^sub>c\<^sub>e \<and> 
       env = flatten_environment env\<^sub>c\<^sub>e \<and> v1 = 3 * v1\<^sub>c\<^sub>e \<and> v2 = 3 * v2\<^sub>c\<^sub>e \<and> vs = flatten_vals vs\<^sub>c\<^sub>e \<and> 
         sfs = flatten_stack sfs\<^sub>c\<^sub>e \<and> p = 2 * p\<^sub>c\<^sub>e" by fastforce
-  with evf_jump have "get_closure (flatten_values h\<^sub>c\<^sub>e) (3 * v2\<^sub>c\<^sub>e) = CELam p' pc'" by simp
+  with evf_jump have "get_closure (flatten_values h\<^sub>c\<^sub>e) (3 * v2\<^sub>c\<^sub>e) = Lam\<^sub>v p' pc'" by simp
   moreover from evf_jump S have "hcontains h\<^sub>c\<^sub>e v2\<^sub>c\<^sub>e" by simp
-  ultimately obtain p\<^sub>c\<^sub>e' where P: "hlookup h\<^sub>c\<^sub>e v2\<^sub>c\<^sub>e = CELam p\<^sub>c\<^sub>e' pc' \<and> p' = 2 * p\<^sub>c\<^sub>e'" by blast
+  ultimately obtain p\<^sub>c\<^sub>e' where P: "hlookup h\<^sub>c\<^sub>e v2\<^sub>c\<^sub>e = Lam\<^sub>v p\<^sub>c\<^sub>e' pc' \<and> p' = 2 * p\<^sub>c\<^sub>e'" by blast
   obtain env\<^sub>c\<^sub>e' p2\<^sub>c\<^sub>e where E: "halloc env\<^sub>c\<^sub>e (v1\<^sub>c\<^sub>e, p\<^sub>c\<^sub>e') = (env\<^sub>c\<^sub>e', p2\<^sub>c\<^sub>e)" by fastforce
-  with evf_jump S P have X: "flatten (CES h\<^sub>c\<^sub>e env\<^sub>c\<^sub>e' vs\<^sub>c\<^sub>e ((Suc p2\<^sub>c\<^sub>e, pc') # sfs\<^sub>c\<^sub>e)) = 
+  with evf_jump S P have X: "flatten (S\<^sub>v h\<^sub>c\<^sub>e env\<^sub>c\<^sub>e' vs\<^sub>c\<^sub>e ((Suc p2\<^sub>c\<^sub>e, pc') # sfs\<^sub>c\<^sub>e)) = 
     FS h env' vs (pc' # Suc (Suc p2) # sfs)" by simp
-  from evf_jump P E have "cd \<tturnstile> CES h\<^sub>c\<^sub>e env\<^sub>c\<^sub>e (v1\<^sub>c\<^sub>e # v2\<^sub>c\<^sub>e # vs\<^sub>c\<^sub>e) ((p\<^sub>c\<^sub>e, Suc pc) # sfs\<^sub>c\<^sub>e) \<leadsto>\<^sub>c\<^sub>e 
-    CES h\<^sub>c\<^sub>e env\<^sub>c\<^sub>e' vs\<^sub>c\<^sub>e ((Suc p2\<^sub>c\<^sub>e, pc') # sfs\<^sub>c\<^sub>e)" by simp
+  from evf_jump P E have "cd \<tturnstile> S\<^sub>v h\<^sub>c\<^sub>e env\<^sub>c\<^sub>e (v1\<^sub>c\<^sub>e # v2\<^sub>c\<^sub>e # vs\<^sub>c\<^sub>e) ((p\<^sub>c\<^sub>e, Suc pc) # sfs\<^sub>c\<^sub>e) \<leadsto>\<^sub>v 
+    S\<^sub>v h\<^sub>c\<^sub>e env\<^sub>c\<^sub>e' vs\<^sub>c\<^sub>e ((Suc p2\<^sub>c\<^sub>e, pc') # sfs\<^sub>c\<^sub>e)" by simp
   with S X show ?case by blast
 qed
 
-theorem completef [simp]: "cd \<tturnstile> \<Sigma>\<^sub>c\<^sub>e \<leadsto>\<^sub>c\<^sub>e \<Sigma>\<^sub>c\<^sub>e' \<Longrightarrow> chained_state \<Sigma>\<^sub>c\<^sub>e \<Longrightarrow> 
+theorem completef [simp]: "cd \<tturnstile> \<Sigma>\<^sub>c\<^sub>e \<leadsto>\<^sub>v \<Sigma>\<^sub>c\<^sub>e' \<Longrightarrow> chained_state \<Sigma>\<^sub>c\<^sub>e \<Longrightarrow> 
   cd \<tturnstile> flatten \<Sigma>\<^sub>c\<^sub>e \<leadsto>\<^sub>f flatten \<Sigma>\<^sub>c\<^sub>e'" 
-proof (induction \<Sigma>\<^sub>c\<^sub>e \<Sigma>\<^sub>c\<^sub>e' rule: evalce.induct)
-  case (evce_pushcon cd pc k h h' v env vs p sfs)
+proof (induction \<Sigma>\<^sub>c\<^sub>e \<Sigma>\<^sub>c\<^sub>e' rule: eval\<^sub>v.induct)
+  case (ev\<^sub>v_pushcon cd pc k h h' v env vs p sfs)
   moreover hence "halloc_list (flatten_values h) [1, k, 0] = (flatten_values h', 3 * v)"
     using flatten_halloc by fastforce
   ultimately show ?case by simp
 next
-  case (evce_pushlam cd pc pc' h p h' v env vs sfs)
+  case (ev\<^sub>v_pushlam cd pc pc' h p h' v env vs sfs)
   moreover hence "halloc_list (flatten_values h) [0, 2 * p, pc'] = (flatten_values h', 3 * v)" 
     using flatten_halloc by fastforce
   ultimately show ?case by simp
 next
-  case (evce_apply cd pc h v2 p' pc' env v1 env' p'' vs p sfs)
+  case (ev\<^sub>v_apply cd pc h v2 p' pc' env v1 env' p'' vs p sfs)
   thus ?case by (simp del: get_closure.simps)
 next
-  case (evce_jump cd pc h v2 p' pc' env v1 env' p'' vs p sfs)
+  case (ev\<^sub>v_jump cd pc h v2 p' pc' env v1 env' p'' vs p sfs)
   thus ?case by (simp del: get_closure.simps)
 qed fastforce+
 
-lemma completef_iter [simp]: "iter (\<tturnstile> cd \<leadsto>\<^sub>c\<^sub>e) \<Sigma>\<^sub>c\<^sub>e \<Sigma>\<^sub>c\<^sub>e' \<Longrightarrow> chained_state \<Sigma>\<^sub>c\<^sub>e \<Longrightarrow>
+lemma completef_iter [simp]: "iter (\<tturnstile> cd \<leadsto>\<^sub>v) \<Sigma>\<^sub>c\<^sub>e \<Sigma>\<^sub>c\<^sub>e' \<Longrightarrow> chained_state \<Sigma>\<^sub>c\<^sub>e \<Longrightarrow>
   iter (\<tturnstile> cd \<leadsto>\<^sub>f) (flatten \<Sigma>\<^sub>c\<^sub>e) (flatten \<Sigma>\<^sub>c\<^sub>e')"
 proof (induction \<Sigma>\<^sub>c\<^sub>e \<Sigma>\<^sub>c\<^sub>e' rule: iter.induct)
   case (iter_step \<Sigma>\<^sub>c\<^sub>e \<Sigma>\<^sub>c\<^sub>e' \<Sigma>\<^sub>c\<^sub>e'')
